Add files via upload

Treiber Stack C11/PSem.thy
@@ -1,5 +1,5 @@
 theory PSem 
-imports Main OpSem
+imports Main OpSem_Proof_Rules
 begin 
 
 datatype object_type = pointer | variable     (*object types to be added, specifically variable?*)
@@ -13,15 +13,215 @@ record posem =
   obj_ctr :: "nat"            (*always increasing with \<forall>i.i\<ge>obj_ctr s \<longrightarrow> A(i) = None*)
                               (* have old pointers *s point to 0, if freed/detached or current value of C - in critical*)
 
-definition "isfree_addr a ps \<equiv> a\<notin>(alloc_addrs ps)"
 
-definition "allocate_object ps loc prov ps' \<equiv> isfree_addr loc ps \<and> prov\<notin>dom(A ps)
- \<and> ps' = ps\<lparr>A := (A ps) (prov:=Some (loc, pointer)),
+definition "codomain_of_A ps \<equiv> \<Union>{{fst(alloc)} | alloc. alloc \<in> ran(A ps)}"
+
+definition "isfree_addr a ps \<equiv> a\<notin>(alloc_addrs ps) "
+
+definition "constant_alloc_ass ps \<equiv> \<forall>loc. (loc \<in> alloc_addrs ps \<longleftrightarrow> loc \<in> codomain_of_A ps)
+                                         \<and>(loc \<notin> alloc_addrs ps \<longleftrightarrow> loc \<notin> codomain_of_A ps)"
+
+definition "Unique_allocs ps \<equiv> \<forall>prov alloc b. (A ps prov) = Some (alloc,b) \<longrightarrow> (\<nexists>prov' b'. 
+                                        prov\<noteq>prov' \<and> (A ps prov') = Some (alloc,b'))"
+
+definition "psem_rules ps \<equiv> Unique_allocs ps \<and> constant_alloc_ass ps"
+
+
+
+
+lemmas alloc_general_lemmas [simp] = codomain_of_A_def isfree_addr_def constant_alloc_ass_def
+                                      Unique_allocs_def psem_rules_def
+
+lemma " psem_rules ps \<Longrightarrow> isfree_addr loc ps \<Longrightarrow> loc\<notin> codomain_of_A ps"
+  using alloc_general_lemmas isfree_addr_def by blast
+
+
+definition "allocate_object ps loc prov ps' typ \<equiv> isfree_addr loc ps \<and> prov \<notin> dom(A ps)
+ \<and> ps' = ps\<lparr>A := (A ps) (prov:=Some (loc, typ)),
             alloc_addrs := (alloc_addrs ps \<union> {loc})\<rparr>"
 
 definition "kill ps prov ps' \<equiv> \<exists>x. (prov \<in> dom(A ps) \<and> Some x = A ps prov 
 \<and> ps' = ps \<lparr> A:= (A ps) (prov:= None),
             alloc_addrs := (alloc_addrs ps - {fst(x)})\<rparr>)"
 
-lemmas posem_lemmas [simp] = isfree_addr_def allocate_object_def kill_def
+lemmas alloc_operation_lemmas [simp] = allocate_object_def kill_def
+
+
+lemma set_alloc_addr_lem1:
+  "allocate_object ps loc prov ps' typ
+  \<Longrightarrow> prov \<notin> dom(A ps)"
+  by auto
+
+lemma set_alloc_addr_lem2:
+  "allocate_object ps loc prov ps' typ
+  \<Longrightarrow> prov \<in> dom(A ps')"
+  by auto
+  
+lemma temp_lemma1:
+  "constant_alloc_ass ps \<Longrightarrow> loc \<in> alloc_addrs ps \<Longrightarrow> loc \<in> codomain_of_A ps"
+  by (simp)
+lemma temp_lemma2:
+  "constant_alloc_ass ps \<Longrightarrow> loc \<in> codomain_of_A ps \<Longrightarrow> loc \<in> alloc_addrs ps"
+  by (simp)
+lemma temp_lemma3:
+  "constant_alloc_ass ps \<Longrightarrow> loc \<notin> alloc_addrs ps \<Longrightarrow> loc \<notin> codomain_of_A ps"
+  by (simp)
+lemma temp_lemma4:
+  "constant_alloc_ass ps \<Longrightarrow> loc \<notin> codomain_of_A ps \<Longrightarrow> loc \<notin> alloc_addrs ps"
+  by (simp)
+
+
+lemma uniqueness_lemma1:
+  "constant_alloc_ass ps \<Longrightarrow> Unique_allocs ps \<Longrightarrow>
+ loca \<in> codomain_of_A ps \<Longrightarrow> 
+ locb \<in> alloc_addrs ps \<Longrightarrow> 
+ prova=provb \<Longrightarrow> fst(the(A ps prova)) = loca \<Longrightarrow> fst(the(A ps provb)) = locb \<Longrightarrow> loca=locb"
+  by (simp)
+
+lemma uniqueness_lemma2:
+  "constant_alloc_ass ps \<Longrightarrow> Unique_allocs ps \<Longrightarrow>
+ \<not>isfree_addr loca ps \<Longrightarrow> 
+ \<not>isfree_addr locb ps \<Longrightarrow>  
+ prova=provb \<Longrightarrow> fst(the(A ps prova)) = loca \<Longrightarrow> fst(the(A ps provb)) = locb \<Longrightarrow> loca=locb"
+  by (simp)
+
+lemma uniqueness_lemma3:
+  "constant_alloc_ass ps \<Longrightarrow>
+ isfree_addr loca ps \<Longrightarrow> 
+ loca \<notin> codomain_of_A ps"
+  by simp
+lemma uniqueness_lemma4:
+  "constant_alloc_ass ps \<Longrightarrow>
+ isfree_addr loca ps \<Longrightarrow> 
+ \<nexists>prova b. A ps prova = Some (loca,b)"
+  apply simp
+  by (metis insertI1 ranI)
+
+lemma uniqueness_lemma5:
+  "constant_alloc_ass ps \<Longrightarrow>
+ isfree_addr loca ps \<Longrightarrow> 
+A ps 1 = Some (1, pointer) \<Longrightarrow>
+A ps 2 = Some (1, variable)
+\<Longrightarrow>
+\<not> Unique_allocs ps "
+  apply simp 
+  by (metis n_not_Suc_n numeral_2_eq_2)
+  
+
+
+
+
+
+
+lemma alloc_step_1:
+  assumes "prov \<notin> dom(A ps)"
+  and "isfree_addr loc ps"
+  and "allocate_object ps loc prov ps' typ"
+shows "prov \<in> dom(A ps')"
+  using assms by simp 
+
+lemma alloc_step_2:
+  assumes "prov \<notin> dom(A ps)"
+  and "isfree_addr loc ps"
+  and "allocate_object ps loc prov ps' typ"
+shows "\<not>(isfree_addr loc ps')"
+  using assms by simp 
+
+lemma alloc_step_3:
+  assumes "prov \<notin> dom(A ps)"
+  and "isfree_addr loc ps"
+  and "allocate_object ps loc prov ps' typ"
+shows "\<not>(isfree_addr loc ps')"
+  using assms by simp 
+
+lemma kill_preserves_structure_1:
+  assumes "constant_alloc_ass ps"
+  and "kill ps prov ps'"
+  and "\<exists>b. A ps prov = Some(loc, b)"
+shows "isfree_addr loc ps'"
+  using assms apply simp
+  apply clarify
+  by auto
+ 
+lemma kill_preserves_structure_2:
+  assumes "constant_alloc_ass ps"
+  and "kill ps prov ps'"
+  and "Unique_allocs ps"
+  and "\<exists>b. A ps prov = Some(loc, b)"
+shows "loc \<notin> codomain_of_A ps'"
+  using assms apply simp
+  apply clarify apply auto 
+  by (metis ComplD insertCI ran_restrictD restrict_complement_singleton_eq)
+  
+lemma kill_preserves_structure_3:
+  assumes "constant_alloc_ass ps"
+  and "kill ps prov ps'"
+  and "Unique_allocs ps"
+  and "\<exists>b. A ps prov = Some(loc, b)"
+shows "\<nexists>prov b. A ps' prov = Some(loc, b)"
+  using assms apply simp
+  apply clarify apply auto 
+  by (metis option.discI)
+
+lemma allocation_preserves_structure:
+  assumes "prov \<notin> dom(A ps)"
+  and "constant_alloc_ass ps"
+  and "isfree_addr loc ps"
+  and "allocate_object ps loc prov ps' typ"
+shows "constant_alloc_ass ps'"
+  using assms apply simp 
+  apply clarify
+  by (smt (z3) assms(1) domIff insert_iff old.prod.inject ran_map_upd singletonD)
+
+lemma kill_preserves_structure:
+  assumes "constant_alloc_ass ps"
+  and "kill ps prov ps'"
+  and "Unique_allocs ps"
+  and "\<exists>b. A ps prov = Some(loc, b)"
+shows "constant_alloc_ass ps'"
+  using assms apply simp
+  apply clarify apply auto
+  apply (smt (z3) Compl_insert Diff_insert_absorb Pair_inject empty_iff fun_upd_same fun_upd_triv fun_upd_upd insertE insert_Diff insert_absorb insert_absorb insert_compr insert_ident insert_iff insert_iff mk_disjoint_insert ranI ran_map_upd restrict_complement_singleton_eq singletonI)
+  apply (metis (no_types, lifting) insert_iff ranI ran_restrictD restrict_complement_singleton_eq)
+  apply (metis ComplD insertCI option.sel ran_restrictD restrict_complement_singleton_eq)
+  apply (metis (no_types, lifting) insert_iff ranI ran_restrictD restrict_complement_singleton_eq)
+  apply (metis ComplD insertCI option.sel ran_restrictD restrict_complement_singleton_eq) 
+  by (smt (z3) Compl_insert Diff_insert_absorb Pair_inject empty_iff fun_upd_same fun_upd_triv fun_upd_upd insertE insert_Diff insert_absorb insert_absorb insert_compr insert_ident insert_iff insert_iff mk_disjoint_insert ranI ran_map_upd restrict_complement_singleton_eq singletonI)
+
+
+lemma allocation_preserves_uniqueness_sup_1:
+  assumes "prov \<notin> dom(A ps)"
+  and "constant_alloc_ass ps"
+  and "Unique_allocs ps"
+  and "isfree_addr loc ps"
+  and "allocate_object ps loc prov ps' typ"
+shows "constant_alloc_ass ps'"
+  using assms allocation_preserves_structure [where ps = ps and ps'=ps'] 
+  by blast
+
+lemma allocation_preserves_uniqueness:
+  assumes "prov \<notin> dom(A ps)"
+  and "constant_alloc_ass ps"
+  and "Unique_allocs ps"
+  and "isfree_addr loc ps"
+  and "allocate_object ps loc prov ps' typ"
+shows "Unique_allocs ps'"
+  using assms apply simp
+  apply clarify apply auto prefer 2
+  apply (metis (no_types) insertI1 ranI)
+  by (metis (no_types) insertI1 ranI)
+
+lemma kill_preserves_uniqueness:
+  assumes "constant_alloc_ass ps"
+  and "kill ps prov ps'"
+  and "Unique_allocs ps"
+  and "\<exists>b. A ps prov = Some(loc, b)"
+shows "Unique_allocs ps'"
+  using assms apply simp
+  apply clarify apply auto 
+  by (metis option.discI)
+  
+
+
+
 end
