Treiber Stack C11/RCU.thy
@@ -1,14 +1,13 @@
 theory RCU
 imports Main PSem
 begin 
-(*weaken invariant own\<^sub>w rather than own\<^sub>R *)
-(*add statement on n:=newint (ABA invariant)*)
 
 
 
 datatype PC = I1 | I2 | I3 | I4 | I5 | I6 | I7 | I8 | I9 | I10 | I11 | I12 | I13 | I14 |  cas_res | finished
             | R1 | R2 | R3 | R4 | R5 
             | S1 | S2 | S3 | S4 | S5 | S6 | S7 
+
 
 
 consts rcu_0 ::address (*first location of rcu array*)
@@ -19,6 +18,8 @@ consts casloc :: nat
 definition "set_T \<equiv> {n . n\<ge>0 \<and> n<T_max}"
 definition "rcu_addrs \<equiv> {n . n\<ge>rcu_0 \<and> n < rcu_0+T_max}"
 definition "something  \<equiv> F \<notin> rcu_addrs \<and> F \<noteq> C \<and> F \<noteq> casloc"
+
+
 
 lemma test:
   assumes "F = i"
@@ -36,8 +37,8 @@ lemma test:
 record mstate =
   pc :: "T \<Rightarrow> PC"
   r :: "T \<Rightarrow> nat \<Rightarrow> nat"        (*local copy of rcu*)
-  n_alloc :: "T \<Rightarrow> bool"        (*now modelled as local pointer allocation - True/False*)
-  s_alloc :: "T \<Rightarrow> bool"        (*now modelled as local pointer allocation - True/False*)
+  n_dec :: "T \<Rightarrow> bool"        (*now modelled as local pointer allocation - True/False*)
+  s_dec :: "T \<Rightarrow> bool"        (*now modelled as local pointer allocation - True/False*)
   v :: "T \<Rightarrow> nat option"        (*now modelled as local value - so M(&v)*)
   n :: "T \<Rightarrow> nat option"        (*now modelled as local value - so M(&n)*)
   s :: "T \<Rightarrow> nat option"        (*now modelled as local value - so M(&s)*)
@@ -68,10 +69,7 @@ definition take_read_ownership :: "T \<Rightarrow> nat \<Rightarrow> mstate \<Ri
 
 definition giveup_readandwrite_ownership :: "T \<Rightarrow> nat \<Rightarrow> mstate \<Rightarrow> mstate" ("givesupRown[_,_]" [200,200])
   where
-  "giveup_readandwrite_ownership t loc ms \<equiv>  if own\<^sub>W ms loc \<noteq> Some t 
-                                            then ms \<lparr> own\<^sub>R := (own\<^sub>R ms) (loc:=own\<^sub>R ms loc - {t}) \<rparr>
-                                            else ms \<lparr> own\<^sub>R := (own\<^sub>R ms) (loc:=own\<^sub>R ms loc - {t}),
-                                                      own\<^sub>W := (own\<^sub>W ms) (loc:=None)\<rparr>"
+  "giveup_readandwrite_ownership t loc ms \<equiv>  ms \<lparr> own\<^sub>R := (own\<^sub>R ms) (loc:=own\<^sub>R ms loc - {t}) \<rparr>"
 
 definition take_write_ownership :: "T \<Rightarrow> nat \<Rightarrow> mstate \<Rightarrow> mstate" ("takesWown[_,_]" [200,200])
   where
@@ -91,13 +89,13 @@ definition v_allocation :: "mstate \<Rightarrow> T \<Rightarrow> mstate \<Righta
 (*int *n*)
 definition int_star_n :: "mstate \<Rightarrow> T \<Rightarrow> mstate \<Rightarrow> bool" ("_ int[*n\<^sub>_] _" [200,200,200])           \<comment>\<open>int *n\<close>
   where
-  "int_star_n ms t ms' \<equiv> ms' = ms \<lparr>n_alloc := (n_alloc ms) (t := True),
+  "int_star_n ms t ms' \<equiv> ms' = ms \<lparr>n_dec := (n_dec ms) (t := True),
                                n := (n ms) (t := None),
                                   pc := (pc ms) (t := I3)\<rparr>"
 (*int *s*)
 definition int_star_s :: "mstate \<Rightarrow> T \<Rightarrow> mstate \<Rightarrow> bool" ("_ int[*s\<^sub>_] _" [200,200,200])           \<comment>\<open>int *s\<close>
   where
-  "int_star_s ms t ms' \<equiv> ms' = ms \<lparr>s_alloc := (s_alloc ms) (t := True),
+  "int_star_s ms t ms' \<equiv> ms' = ms \<lparr>s_dec := (s_dec ms) (t := True),
                                s := (s ms) (t := None),
                                   pc := (pc ms) (t := I4) \<rparr>"
 
@@ -107,11 +105,42 @@ definition int_star_s :: "mstate \<Rightarrow> T \<Rightarrow> mstate \<Rightarr
 (*******   n = new int  **********)
 definition new_int :: "mstate \<Rightarrow> posem \<Rightarrow> T \<Rightarrow> mstate \<Rightarrow> posem \<Rightarrow> bool" ( "_ _ n:=newint _ _ _" [200,200,200,200,200])
   where
-  "new_int ms ps t ms' ps' \<equiv> (\<exists> loc prov . (allocate_object ps loc prov ps' 
+  "new_int ms ps t ms' ps' \<equiv>  (\<exists>loc prov. (allocate_object ps loc prov ps' variable 
                                     \<and> ms' = ms \<lparr>n := (n ms) (t := Some loc),
                                                  own\<^sub>R := (own\<^sub>R ms) (loc:=own\<^sub>R ms loc \<union> {t}),
                                                  own\<^sub>W := (own\<^sub>W ms) (loc:=Some t),
                                                    pc := (pc ms) (t := I5) \<rparr>))"
+
+lemma switch:
+  "prov\<notin> dom(A ps) \<longrightarrow> A ps prov = None"
+  by auto
+
+lemma switch2:
+  "n ms t = None \<Longrightarrow> \<exists>prov loc. (allocate_object ps loc prov ps' variable  
+                                    \<and> ms' = ms \<lparr>n := (n ms) (t := Some loc),
+                                             own\<^sub>R := (own\<^sub>R ms) (loc:=own\<^sub>R ms loc \<union> {t}),
+                                             own\<^sub>W := (own\<^sub>W ms) (loc:=Some t),
+                                               pc := (pc ms) (t := I5) \<rparr>) 
+      \<Longrightarrow> n ms' t\<noteq> None"
+  apply(simp add:new_int_def) apply clarify
+  by simp
+
+lemma switch3:
+  "n ms t = None \<Longrightarrow> \<exists>prov loc. (allocate_object ps loc prov ps' variable  
+                                    \<and> ms' = ms \<lparr>n := (n ms) (t := Some loc),
+                                             own\<^sub>R := (own\<^sub>R ms) (loc:=own\<^sub>R ms loc \<union> {t}),
+                                             own\<^sub>W := (own\<^sub>W ms) (loc:=Some t),
+                                               pc := (pc ms) (t := I5) \<rparr>) 
+    \<Longrightarrow> own\<^sub>W ms' (the(n ms' t)) =Some  t"
+  apply(simp add:new_int_def) apply clarify 
+  by clarsimp
+
+
+
+
+
+
+
 
 
 (*******   s = C   **********)
@@ -126,12 +155,17 @@ definition get_C_val :: "mstate \<Rightarrow> surrey_state \<Rightarrow> T \<Rig
                        pc := (pc ms) (t := I9),
                      own\<^sub>R := (own\<^sub>R ms) ((snd(FAAZ t w \<sigma> ts')):=own\<^sub>R ms (snd(FAAZ t w \<sigma> ts')) \<union> {t})\<rparr>)" 
 
+
+
+
+
+
+
 (*******   v=*s   **********)
 definition get_s :: "mstate \<Rightarrow> surrey_state \<Rightarrow> T  \<Rightarrow> mstate \<Rightarrow> surrey_state \<Rightarrow> bool" ( "_ _ v:=*s _ _ _" [200,200,200,200,200])
   where
   "get_s ms \<sigma> t ms' \<sigma>' \<equiv>  (\<exists>z.  \<sigma> [z \<leftarrow> the (s ms t)]\<^sub>t \<sigma>'
                                       \<and> ms' = ms \<lparr> v := (v ms) (t := Some z),
-                                                      own\<^sub>R := ( own\<^sub>R ms ) (z := own\<^sub>R ms z \<union> {t}),
                                                       pc := (pc ms) (t := I10)\<rparr>)" 
 
 
@@ -179,10 +213,8 @@ definition exit_rcu :: "posem \<Rightarrow> surrey_state \<Rightarrow> T \<Right
 
 definition setup_r :: "mstate \<Rightarrow> T \<Rightarrow>  mstate \<Rightarrow> bool" ("_ r[N]:={0} _ _" [200])    \<comment>\<open>r[N] = {0}\<close>
   where
-  "setup_r  ms t ms' \<equiv> ms' = ms\<lparr>r := \<lambda> x n. if x = t then 0 else r ms x n,
-                                  pc := (pc ms) (t := S2)\<rparr>"
-
-
+  "setup_r  ms t ms' \<equiv> ms' = ms \<lparr> r := (r ms) (t := \<lambda> i . 0),
+                                 pc := (pc ms) (t := S2)\<rparr>"
 
 
 
@@ -208,9 +240,10 @@ definition take_rd_cap :: "L \<Rightarrow> T \<Rightarrow> mstate \<Rightarrow> 
 
 definition insert_address :: " mstate \<Rightarrow> T \<Rightarrow> nat \<Rightarrow> mstate \<Rightarrow> bool" ("_ insert[detached[_],_] _" [200,200,200,200])    \<comment>\<open>insert(_, s)\<close>
   where
-  "insert_address ms loc t ms' \<equiv> ms' = ms\<lparr> det := (det ms) (t:= (((det ms) t) @ [loc])),
+  "insert_address ms t loc ms' \<equiv> ms' = ms\<lparr> det := (det ms) (t:= (((det ms) t) @ [loc])),
                                             pc := (pc ms) (t := R2), 
-                                             s_alloc := (s_alloc ms) (t := False)\<rparr>"
+                                             s_dec := (s_dec ms) (t := False),
+                                             s := (s ms) (t := None)\<rparr>"
 
 
 definition nondet :: "mstate \<Rightarrow> T \<Rightarrow> bool \<Rightarrow> mstate \<Rightarrow> bool" ("_ nondet[_,_] _" [200,200,200,200])    \<comment>\<open>nondet()\<close>
@@ -234,9 +267,10 @@ definition cas_step_rcu :: "mstate \<Rightarrow> surrey_state \<Rightarrow>T \<R
        \<sigma>' = fst(CAS t w cv nv \<sigma> ts')    
        \<and> 
 (snd(CAS t w cv nv \<sigma> ts') = True \<longrightarrow>(ms' = ms\<lparr>CAS_succ := (CAS_succ ms) (t := snd(CAS t w cv nv \<sigma> ts')),
+                                                 n_dec := (n_dec ms) (t := False),
                                                   own\<^sub>W := (own\<^sub>W ms) (cv:=Some t),        \<comment>\<open>acquire wr_cap on location\<close>
                                                   own\<^sub>W := (own\<^sub>W ms) (nv:=None),          \<comment>\<open>let go of wr_cap on location\<close>
-                                                   pc := (pc ms) (t := cas_res)\<rparr>))
+                                                   pc  := (pc ms) (t := cas_res)\<rparr>))
        \<and> 
 (snd(CAS t w cv nv \<sigma> ts') = False \<longrightarrow>(ms' = ms\<lparr>CAS_succ := (CAS_succ ms) (t := snd(CAS t w cv nv \<sigma> ts')),
                                                    pc := (pc ms) (t := cas_res)\<rparr>))"           
@@ -272,11 +306,11 @@ definition repetition :: "T \<Rightarrow> bool \<Rightarrow> mstate \<Rightarrow
 
 definition nallocdef :: "T \<Rightarrow> bool \<Rightarrow> mstate \<Rightarrow> mstate" ( "n[_]:=_" [200,200])
   where
-  "nallocdef t b ms \<equiv>  ms \<lparr> n_alloc := (n_alloc ms) (t:=b) \<rparr> "
+  "nallocdef t b ms \<equiv>  ms \<lparr> n_dec := (n_dec ms) (t:=b) \<rparr> "
 
 definition sallocdef :: "T \<Rightarrow> bool \<Rightarrow> mstate \<Rightarrow> mstate" ( "s[_]:=_" [200,200])
   where
-  "sallocdef t b ms \<equiv>  ms \<lparr> s_alloc := (s_alloc ms) (t:=b) \<rparr> "
+  "sallocdef t b ms \<equiv>  ms \<lparr> s_dec := (s_dec ms) (t:=b) \<rparr> "
 
 definition SC_fence :: "surrey_state \<Rightarrow> T \<Rightarrow> surrey_state \<Rightarrow> bool " ("_ Fence _ _" [200,200,200])
   where
@@ -291,7 +325,7 @@ definition SC_fence :: "surrey_state \<Rightarrow> T \<Rightarrow> surrey_state 
 
 
 lemmas abbr = v_allocation_def int_star_n_def int_star_s_def
-                new_int_def get_C_val_def get_s_def writeto_star_n_def
+                new_int_def get_s_def writeto_star_n_def
                 pop_address_def
                 load_rcu_to_r_def 
                 enter_rcu_def exit_rcu_def
@@ -321,9 +355,10 @@ case pcr of
 |  R4 \<Rightarrow> if (det ms t \<noteq> [])
             then ms' = (pc[t]:=R5)  ms  \<and> ps = ps' \<and> \<sigma> =\<sigma>'  
             else ms' = (pc[t]:=I13) ms  \<and> ps = ps' \<and> \<sigma> =\<sigma>'     \<comment>\<open> return to inc() \<close>
+\<comment>\<open> \<close>
 |  R5 \<Rightarrow> (ms ps free[pop[detached[t]]] ms' ps')  \<and> \<sigma> =\<sigma>'                  \<comment>\<open> ownW ps hd(det ps t) := None \<close>
-
-|  S1 \<Rightarrow> (ms r[N]:={0} t ms) \<and> ps = ps'  \<and> \<sigma> = \<sigma>'
+\<comment>\<open> \<close>
+|  S1 \<Rightarrow> (ms r[N]:={0} t ms') \<and> ps = ps'  \<and> \<sigma> = \<sigma>'
 |  S2 \<Rightarrow> if (CTRsync\<^sub>1 ms t < T_max)
             then ms' = (CTRsync\<^sub>1[t]++ \<circ> pc[t]:=S3) ms \<and> ps = ps' \<and> \<sigma> =\<sigma>'
             else ms' = (pc[t]:=S4) ms \<and> ps = ps' \<and> \<sigma> =\<sigma>'
@@ -353,8 +388,8 @@ case pcr of
 |  I10 \<Rightarrow> (ms \<sigma> *n:=newv t ms' \<sigma>')   \<and> ps = ps'                  \<comment>\<open> (ownW ps n) = t \<close>
 |  I11 \<Rightarrow> cas_step_rcu ms \<sigma> t C (the (s ms t)) (the (n ms t)) ms' \<sigma>' \<and> ps = ps'           \<comment>\<open> swaps wr cap from n to s\<close>
 |  cas_res \<Rightarrow> if CAS_succ ms t 
-            then (ms' = (pc[t]:=I12) ms)
-            else (ms' = (pc[t]:=I6 \<circ> repeat[t]:=True) ms)
+            then (ms' = (pc[t]:=I12) ms) \<and> ps = ps' \<and> \<sigma> = \<sigma>'
+            else (ms' = (pc[t]:=I6 \<circ> repeat[t]:=True) ms) \<and> ps = ps' \<and> \<sigma> = \<sigma>'
 |  I12 \<Rightarrow> (ps \<sigma> rcuexit[] t ps' \<sigma>') \<and> (ms' = ((pc[t]:=R1 \<circ> n[t]:=False \<circ> givesupRown[t,the (n ms t)])) ms)  \<comment>\<open> lets go of raw cap on n\<close>
         \<comment>\<open>reclaim(s)\<close>                                            \<comment>\<open> (ownW ps s) = t \<close>            \<comment>\<open> lets go of raw cap on s\<close>
 |  I13 \<Rightarrow> (ms' = (pc[t]:=I14) ms) \<and> \<sigma> = \<sigma>' \<and> ps = ps'   
@@ -362,13 +397,17 @@ case pcr of
 | finished \<Rightarrow> ms = ms' \<and> ps=ps' \<and> \<sigma>=\<sigma>'
 " 
 
+lemma "n ms' t \<noteq> i \<Longrightarrow> (SOME loc. (the(n ms' t) = loc)) \<equiv> the(n ms' t)"
+  by simp
+  
+
+  
+lemma " \<exists> x. (x=2 \<and> x = p) \<Longrightarrow>  (SOME x.  x)  \<equiv> p=2 "
+  by (simp add: some_equality)
 
 
 
-(*------- todo ----------
-  r :: "T \<Rightarrow> nat \<Rightarrow> nat"          
-  det :: "T \<Rightarrow> L list"        
--------------------------*)
+
 
 
 
@@ -377,14 +416,17 @@ definition "Wcap ms t addrs \<equiv> \<forall>i. (i\<in>addrs) \<longleftrightar
 
 definition "inlist a lst \<equiv> \<exists>j.(j<length(lst) \<and> lst!j = a)"
 definition "detaddrs ms t \<equiv> {i. inlist i (det ms t)}"
+definition "tail_detaddrs ms t \<equiv> {i. inlist i (det ms t)}"
 definition "n_pointer ms t\<equiv> the(n ms t)"
 definition "s_pointer ms t\<equiv> the(s ms t)"
 definition "s_and_n ms t \<equiv> {n_pointer ms t,s_pointer ms t}"
 definition "just_n ms t \<equiv> {n_pointer ms t}"
 definition "just_s ms t \<equiv> {s_pointer ms t}"
 
+(*\<forall>t loc. t\<le>T_max \<and> loc\<noteq>s_t \<and> loc\<noteq>n_t \<and> loc \<notin> detaddrs ms t \<and> loc\<noteq>C \<and> loc\<noteq>rcu[t]\<longrightarrow> loc\<in>free *)
+(*\<forall>loc. loc\<in>free \<longrightarrow> own\<^sub>R ms loc = {}*)
 lemmas names [simp] = n_pointer_def s_pointer_def s_and_n_def just_n_def just_s_def
-                      inlist_def detaddrs_def
+                      inlist_def detaddrs_def tail_detaddrs_def
 lemmas names_2      = Rcap_def Wcap_def
 
 
@@ -393,18 +435,28 @@ lemmas names_2      = Rcap_def Wcap_def
 definition "addr_allocated ms ps \<equiv> \<forall>addr t . addr \<in> detaddrs ms t \<longrightarrow> 
                                  (\<exists>prov. (A ps prov = Some (addr, pointer)))"
 
-definition "nptr_true_imp ms ps \<equiv> \<forall>t . (n_alloc ms t = True \<and> n ms t\<noteq>None) \<longrightarrow>
+definition "nptr_true_imp ms ps \<equiv> \<forall>t . (n_dec ms t = True \<and> n ms t\<noteq>None) \<longrightarrow>
                           (\<exists>prov. (A ps prov = Some (the (n ms t), pointer)))"
 
-definition "sptr_true_imp ms ps \<equiv> \<forall>t . (s_alloc ms t = True \<and> s ms t\<noteq>None) \<longrightarrow>
+definition "sptr_true_imp ms ps \<equiv> \<forall>t . (s_dec ms t = True \<and> s ms t\<noteq>None) \<longrightarrow>
                           (\<exists>prov. (A ps prov = Some (the (s ms t), pointer)))"
+
+(*-----------observation lemmas --------------*)
+
+
+
+
 
 
 (*------- careful observation of preCond per thread ----------*)
 definition "pre_I1 ms t \<equiv>
-                         Rcap ms t (detaddrs ms t) \<and> Wcap ms t (detaddrs ms t)"
+                         Rcap ms t (detaddrs ms t) \<and> Wcap ms t (detaddrs ms t)
+                       \<and> n ms t = None 
+                       \<and> n_dec ms t = False
+"
+
 (* s ms t = None
-                        \<and> n ms t = None 
+                        
                         \<and> v ms t = None
                         \<and> s ms t = False 
                         \<and> n ms t = False 
@@ -413,18 +465,24 @@ definition "pre_I1 ms t \<equiv>
                         \<and> nondet_val ms t = False \<and> CAS_succ ms t = False \<and> repeat ms t = False
                         \<and> *)
 definition "pre_I2 ms t \<equiv>
-                          Rcap ms t (detaddrs ms t) \<and> Wcap ms t (detaddrs ms t)"
+                          Rcap ms t (detaddrs ms t) \<and> Wcap ms t (detaddrs ms t)
+                        \<and> n ms t = None 
+                        \<and> n_dec ms t = True
+"
 (*s ms t = None 
                         \<and> n ms t = None 
                         \<and> v ms t = None
                         \<and> s ms t = False 
-                        \<and> n ms t = False 
+                        \<and> n_dec ms t = False 
                         \<and> CTRsync\<^sub>1 ms t = 0 \<and> CTRsync\<^sub>2 ms t = 0 
                         \<and> res ms t = 0 \<and> reg ms t = 0
                         \<and> nondet_val ms t = False \<and> CAS_succ ms t = False \<and> repeat ms t = False
                         \<and> *)
 definition "pre_I3 ms t \<equiv>
-                           Rcap ms t (detaddrs ms t) \<and> Wcap ms t (detaddrs ms t)"
+                         Rcap ms t (detaddrs ms t) \<and> Wcap ms t (detaddrs ms t)
+                       \<and> n ms t = None 
+                       \<and> n_dec ms t = True
+"
 (*s ms t = None 
                         \<and> n ms t = None 
                         \<and> v ms t = None
@@ -435,7 +493,10 @@ definition "pre_I3 ms t \<equiv>
                         \<and> nondet_val ms t = False \<and> CAS_succ ms t = False \<and> repeat ms t = False
                         \<and>*)
 definition "pre_I4 ms t \<equiv>
-                          Rcap ms t (detaddrs ms t) \<and> Wcap ms t (detaddrs ms t)"
+                          Rcap ms t (detaddrs ms t) \<and> Wcap ms t (detaddrs ms t)
+                       \<and> n ms t = None 
+                       \<and> n_dec ms t = True
+"
 (*s ms t = None
                         \<and> n ms t = None
                         \<and> v ms t = None
@@ -446,7 +507,10 @@ definition "pre_I4 ms t \<equiv>
                         \<and> nondet_val ms t = False \<and> CAS_succ ms t = False \<and> repeat ms t = False
                         \<and> *)
 definition "pre_I5 ms t \<equiv>
-                           Rcap ms t (detaddrs ms t \<union> just_n ms t) \<and> Wcap ms t (detaddrs ms t \<union> just_n ms t)"
+                           Rcap ms t (detaddrs ms t \<union> just_n ms t) \<and> Wcap ms t (detaddrs ms t \<union> just_n ms t)
+                       \<and> n ms t \<noteq> None 
+                       \<and> n_dec ms t = True
+"
 (*s ms t = None
                         \<and> (\<exists>i. n ms t = Some i)
                         \<and> v ms t = None
@@ -457,9 +521,13 @@ definition "pre_I5 ms t \<equiv>
                         \<and> nondet_val ms t = False \<and> CAS_succ ms t = False \<and> repeat ms t = False
                         \<and>*)
 definition "pre_I6 ms t \<equiv>
-                           Wcap ms t (detaddrs ms t \<union> just_n ms t)"
-(*(repeat ms t  \<longrightarrow> (\<exists>j k. s ms t = Some j \<and> v ms t = Some k)
-                                          \<and> Rcap ms t (detaddrs ms t \<union> s_and_n ms t))
+                         Wcap ms t (detaddrs ms t \<union> just_n ms t) 
+                \<and>  repeat ms t  \<longrightarrow>(s ms t \<noteq> None \<and> Rcap ms t (detaddrs ms t \<union> s_and_n ms t))
+                \<and> \<not>repeat ms t  \<longrightarrow>(s ms t = None \<and> Rcap ms t (detaddrs ms t \<union> just_n ms t))
+                       \<and> n ms t \<noteq> None 
+                       \<and> n_dec ms t = True
+"
+(*(repeat ms t  \<longrightarrow> (\<exists>j k. s ms t = Some j \<and> v ms t = Some k))
                         \<and> (\<not>repeat ms t \<longrightarrow> s ms t = None \<and> v ms t = None
                                           \<and> Rcap ms t (detaddrs ms t \<union> just_n ms t))
                         \<and> (\<exists>i. n ms t = Some i)
@@ -470,7 +538,10 @@ definition "pre_I6 ms t \<equiv>
                         \<and> nondet_val ms t = False \<and> CAS_succ ms t = False 
                         \<and>*)
 definition "pre_I7 ms t \<equiv>
-                          Rcap ms t (detaddrs ms t \<union> just_n ms t) \<and> Wcap ms t (detaddrs ms t \<union> just_n ms t)"
+                          Rcap ms t (detaddrs ms t \<union> just_n ms t) \<and> Wcap ms t (detaddrs ms t \<union> just_n ms t)
+                       \<and> n ms t \<noteq> None 
+                       \<and> n_dec ms t = True
+"
 (*(\<not>repeat ms t \<longrightarrow> s ms t = None \<and> v ms t = None)
                         \<and> (repeat ms t \<longrightarrow> (\<exists>j k. s ms t = Some j \<and> v ms t = Some k))
                         \<and> (\<exists>i. n ms t = Some i)
@@ -481,7 +552,10 @@ definition "pre_I7 ms t \<equiv>
                         \<and> nondet_val ms t = False \<and> CAS_succ ms t = False 
                         \<and> *)
 definition "pre_I8 ms t \<equiv> 
-                           Rcap ms t (detaddrs ms t \<union> just_n ms t) \<and> Wcap ms t (detaddrs ms t \<union> just_n ms t)"
+                           Rcap ms t (detaddrs ms t \<union> just_n ms t) \<and> Wcap ms t (detaddrs ms t \<union> just_n ms t)
+                       \<and> n ms t \<noteq> None 
+                       \<and> n_dec ms t = True
+"
 (*(\<not>repeat ms t \<longrightarrow> s ms t = None \<and> v ms t = None)
                         \<and> (repeat ms t \<longrightarrow> (\<exists>j k. s ms t = Some j \<and> v ms t = Some k))
                         \<and> (\<exists>i. n ms t = Some i)
@@ -492,7 +566,10 @@ definition "pre_I8 ms t \<equiv>
                         \<and> nondet_val ms t = False \<and> CAS_succ ms t = False
                         \<and>*)
 definition "pre_I9 ms t \<equiv> 
-                           Rcap ms t (detaddrs ms t \<union> s_and_n ms t) \<and> Wcap ms t (detaddrs ms t \<union> just_n ms t)"
+                           Rcap ms t (detaddrs ms t \<union> s_and_n ms t) \<and> Wcap ms t (detaddrs ms t \<union> just_n ms t)
+                       \<and> n ms t \<noteq> None 
+                       \<and> n_dec ms t = True
+"
 (*(\<not>repeat ms t \<longrightarrow>  v ms t = None)
                         \<and> (repeat ms t \<longrightarrow> (\<exists>k. v ms t = Some k))
                         \<and> (\<exists>j. s ms t = Some j)
@@ -504,7 +581,10 @@ definition "pre_I9 ms t \<equiv>
                         \<and> nondet_val ms t = False \<and> CAS_succ ms t = False 
                         \<and>*)
 definition "pre_I10 ms t \<equiv>
-                           Rcap ms t (detaddrs ms t \<union> s_and_n ms t) \<and> Wcap ms t (detaddrs ms t \<union> just_n ms t)"
+                           Rcap ms t (detaddrs ms t \<union> s_and_n ms t) \<and> Wcap ms t (detaddrs ms t \<union> just_n ms t)
+                       \<and> n ms t \<noteq> None 
+                       \<and> n_dec ms t = True
+"
 (*(\<exists>j. s ms t = Some j)
                         \<and> (\<exists>i. n ms t = Some i)
                         \<and> (\<exists>k. v ms t = Some k)
@@ -515,7 +595,10 @@ definition "pre_I10 ms t \<equiv>
                         \<and> nondet_val ms t = False \<and> CAS_succ ms t = False
                         \<and>*)
 definition "pre_I11 ms t \<equiv>
-                          Rcap ms t (detaddrs ms t \<union> s_and_n ms t) \<and> Wcap ms t (detaddrs ms t \<union> just_n ms t)"
+                          Rcap ms t (detaddrs ms t \<union> s_and_n ms t) \<and> Wcap ms t (detaddrs ms t \<union> just_n ms t)
+                       \<and> n ms t \<noteq> None 
+                       \<and> n_dec ms t = True
+"
 (*(\<exists>j. s ms t = Some j)
                         \<and> (\<exists>i. n ms t = Some i)
                         \<and> (\<exists>k. v ms t = Some k)
@@ -526,8 +609,12 @@ definition "pre_I11 ms t \<equiv>
                         \<and> nondet_val ms t = False \<and> CAS_succ ms t = False
                         \<and> *)
 definition "pre_cas_res ms t \<equiv>
-                          (CAS_succ ms t \<longrightarrow> Rcap ms t (detaddrs ms t \<union> s_and_n ms t) \<and> Wcap ms t (detaddrs ms t \<union> just_s ms t))
-                        \<and> (\<not>CAS_succ ms t\<longrightarrow> Rcap ms t (detaddrs ms t \<union> s_and_n ms t) \<and> Wcap ms t (detaddrs ms t \<union> just_n ms t))"
+                          (CAS_succ ms t \<longrightarrow> Rcap ms t (detaddrs ms t \<union> s_and_n ms t) \<and> Wcap ms t (detaddrs ms t \<union> just_s ms t)
+                       \<and> n_dec ms t)
+                        \<and> (\<not>CAS_succ ms t\<longrightarrow> Rcap ms t (detaddrs ms t \<union> s_and_n ms t) \<and> Wcap ms t (detaddrs ms t \<union> just_n ms t)
+                       \<and> \<not>n_dec ms t)
+                       \<and> n ms t \<noteq> None 
+"
 (*(\<exists>j. s ms t = Some j)
                         \<and> (\<exists>i. n ms t = Some i)
                         \<and> (\<exists>k. v ms t = Some k)
@@ -538,7 +625,10 @@ definition "pre_cas_res ms t \<equiv>
                         \<and> nondet_val ms t = False 
                         \<and> *)
 definition "pre_I12 ms t \<equiv>
-                           Rcap ms t (detaddrs ms t \<union> s_and_n ms t) \<and> Wcap ms t (detaddrs ms t \<union> just_s ms t)"
+                           Rcap ms t (detaddrs ms t \<union> s_and_n ms t) \<and> Wcap ms t (detaddrs ms t \<union> just_s ms t)
+                       \<and> \<not>n_dec ms t
+                       \<and> n ms t \<noteq> None 
+"
 (*(\<exists>j. s ms t = Some j)
                         \<and> (\<exists>i. n ms t = Some i)
                         \<and> (\<exists>k. v ms t = Some k)
@@ -550,7 +640,10 @@ definition "pre_I12 ms t \<equiv>
                         \<and>*)
 \<comment>\<open> start to reclaim() \<close>
 definition "pre_I13 ms t \<equiv>
-                          Rcap ms t (detaddrs ms t) \<and> Wcap ms t (detaddrs ms t)"
+                          Rcap ms t (detaddrs ms t) \<and> Wcap ms t (detaddrs ms t)
+                       \<and> \<not>n_dec ms t
+                       \<and> n ms t \<noteq> None 
+"
 (*(\<exists>j. s ms t = Some j)
                         \<and> (\<exists>i. n ms t = Some i)
                         \<and> (\<exists>k. v ms t = Some k)
@@ -561,7 +654,10 @@ definition "pre_I13 ms t \<equiv>
                         \<and> nondet_val ms t = False \<and> CAS_succ ms t = True
                         \<and> *)
 definition "pre_I14 ms t \<equiv>
-                           Rcap ms t (detaddrs ms t) \<and> Wcap ms t (detaddrs ms t)"
+                           Rcap ms t (detaddrs ms t) \<and> Wcap ms t (detaddrs ms t)
+                       \<and> \<not>n_dec ms t
+                       \<and> n ms t \<noteq> None 
+"
 (*(\<exists>j. s ms t = Some j)
                         \<and> (\<exists>i. n ms t = Some i)
                         \<and> (\<exists>k. v ms t = Some k)
@@ -574,7 +670,10 @@ definition "pre_I14 ms t \<equiv>
 
 
 definition "pre_R1 ms t \<equiv>  
-                           Rcap ms t (detaddrs ms t \<union> just_s ms t) \<and> Wcap ms t (detaddrs ms t \<union> just_s ms t)"
+                           Rcap ms t (detaddrs ms t \<union> just_s ms t) \<and> Wcap ms t (detaddrs ms t \<union> just_s ms t)
+                       \<and> \<not>n_dec ms t
+                       \<and> n ms t \<noteq> None 
+"
 (*(\<exists>j. s ms t = Some j)
                         \<and> (\<exists>i. n ms t = Some i)
                         \<and> (\<exists>k. v ms t = Some k)
@@ -585,7 +684,10 @@ definition "pre_R1 ms t \<equiv>
                         \<and> nondet_val ms t = False \<and> CAS_succ ms t = True
                         \<and>*)
 definition "pre_R2 ms t \<equiv>
-                           Rcap ms t (detaddrs ms t) \<and> Wcap ms t (detaddrs ms t)"
+                           Rcap ms t (detaddrs ms t) \<and> Wcap ms t (detaddrs ms t)
+                       \<and> \<not>n_dec ms t
+                       \<and> n ms t \<noteq> None 
+"
 (*(\<exists>j. s ms t = Some j)
                         \<and> (\<exists>i. n ms t = Some i)
                         \<and> (\<exists>k. v ms t = Some k)
@@ -597,7 +699,10 @@ definition "pre_R2 ms t \<equiv>
                         \<and> nondet_val ms t = False \<and> CAS_succ ms t = True
                         \<and>*)
 definition "pre_R3 ms t \<equiv>
-                           Rcap ms t (detaddrs ms t) \<and> Wcap ms t (detaddrs ms t)"
+                           Rcap ms t (detaddrs ms t) \<and> Wcap ms t (detaddrs ms t)
+                       \<and> \<not>n_dec ms t
+                       \<and> n ms t \<noteq> None 
+"
 (*(\<exists>j. s ms t = Some j)
                         \<and> (\<exists>i. n ms t = Some i)
                         \<and> (\<exists>k. v ms t = Some k)
@@ -611,7 +716,10 @@ definition "pre_R3 ms t \<equiv>
 \<comment>\<open> start to sync() \<close>
 \<comment>\<open> or return to inc() \<close>
 definition "pre_R4 ms t \<equiv>  
-                           Rcap ms t (detaddrs ms t) \<and> Wcap ms t (detaddrs ms t)"
+                           Rcap ms t (detaddrs ms t) \<and> Wcap ms t (detaddrs ms t)
+                       \<and> \<not>n_dec ms t
+                       \<and> n ms t \<noteq> None 
+"
 (*(\<exists>j. s ms t = Some j)
                         \<and> (\<exists>i. n ms t = Some i)
                         \<and> (\<exists>k. v ms t = Some k)
@@ -623,7 +731,10 @@ definition "pre_R4 ms t \<equiv>
                         \<and>*)
 \<comment>\<open> return to inc() \<close>
 definition "pre_R5 ms t \<equiv>
-                           Rcap ms t (detaddrs ms t) \<and> Wcap ms t (detaddrs ms t)"
+                           Rcap ms t (detaddrs ms t) \<and> Wcap ms t (detaddrs ms t)
+                       \<and> \<not>n_dec ms t
+                       \<and> n ms t \<noteq> None 
+"
 (*(\<exists>j. s ms t = Some j)
                         \<and> (\<exists>i. n ms t = Some i)
                         \<and> (\<exists>k. v ms t = Some k)
@@ -637,7 +748,10 @@ definition "pre_R5 ms t \<equiv>
 
 
 definition "pre_S1 ms t \<equiv>  
-                           Rcap ms t (detaddrs ms t) \<and> Wcap ms t (detaddrs ms t)"
+                           Rcap ms t (detaddrs ms t) \<and> Wcap ms t (detaddrs ms t)
+                       \<and> \<not>n_dec ms t
+                       \<and> n ms t \<noteq> None 
+"
 (*(\<exists>j. s ms t = Some j)
                         \<and> (\<exists>i. n ms t = Some i)
                         \<and> (\<exists>k. v ms t = Some k)
@@ -649,7 +763,10 @@ definition "pre_S1 ms t \<equiv>
                         \<and> nondet_val ms t = True \<and> CAS_succ ms t = True 
                         \<and>*)
 definition "pre_S2 ms t \<equiv>
-                           Rcap ms t (detaddrs ms t) \<and> Wcap ms t (detaddrs ms t)"
+                           Rcap ms t (detaddrs ms t) \<and> Wcap ms t (detaddrs ms t)
+                       \<and> \<not>n_dec ms t
+                       \<and> n ms t \<noteq> None 
+"
 (*(\<exists>j. s ms t = Some j)
                         \<and> (\<exists>i. n ms t = Some i)
                         \<and> (\<exists>k. v ms t = Some k)
@@ -662,7 +779,10 @@ definition "pre_S2 ms t \<equiv>
                         \<and> (\<forall>i. (i>CTRsync\<^sub>1 ms t \<and> i\<le>T_max) \<longrightarrow> r ms t i = 0)        \<comment> \<open>local rcu register\<close>
                         \<and>*)
 definition "pre_S3 ms t \<equiv>
-                           Rcap ms t (detaddrs ms t) \<and> Wcap ms t (detaddrs ms t)"
+                           Rcap ms t (detaddrs ms t) \<and> Wcap ms t (detaddrs ms t)
+                       \<and> \<not>n_dec ms t
+                       \<and> n ms t \<noteq> None 
+"
 (*(\<exists>j. s ms t = Some j)
                         \<and> (\<exists>i. n ms t = Some i)
                         \<and> (\<exists>k. v ms t = Some k)
@@ -675,7 +795,10 @@ definition "pre_S3 ms t \<equiv>
                         \<and> (\<forall>i. (i\<ge>CTRsync\<^sub>1 ms t \<and> i\<le>T_max) \<longrightarrow> r ms t i = 0)        \<comment> \<open>local rcu register\<close>
                         \<and>*)
 definition "pre_S4 ms t \<equiv>
-                           Rcap ms t (detaddrs ms t) \<and> Wcap ms t (detaddrs ms t)"
+                           Rcap ms t (detaddrs ms t) \<and> Wcap ms t (detaddrs ms t)
+                       \<and> \<not>n_dec ms t
+                       \<and> n ms t \<noteq> None 
+"
 (*(\<exists>j. s ms t = Some j)
                         \<and> (\<exists>i. n ms t = Some i)
                         \<and> (\<exists>k. v ms t = Some k)
@@ -688,7 +811,10 @@ definition "pre_S4 ms t \<equiv>
                         \<and> (\<forall>i. (i\<ge>CTRsync\<^sub>1 ms t \<and> i\<le>T_max) \<longrightarrow> r ms t i = 0)        \<comment> \<open>careful, here is smth to do with observations in wm\<close>
                         \<and>*)
 definition "pre_S5 ms t \<equiv>
-                           Rcap ms t (detaddrs ms t) \<and> Wcap ms t (detaddrs ms t)"
+                           Rcap ms t (detaddrs ms t) \<and> Wcap ms t (detaddrs ms t)
+                       \<and> \<not>n_dec ms t
+                       \<and> n ms t \<noteq> None 
+"
 (*(\<exists>j. s ms t = Some j)
                         \<and> (\<exists>i. n ms t = Some i)
                         \<and> (\<exists>k. v ms t = Some k)
@@ -701,7 +827,10 @@ definition "pre_S5 ms t \<equiv>
                         \<and> (\<forall>i. (i\<ge>CTRsync\<^sub>1 ms t \<and> i\<le>T_max) \<longrightarrow> r ms t i = 0)        \<comment> \<open>careful, here is smth to do with observations in wm\<close>
                         \<and>*)
 definition "pre_S6 ms t \<equiv>
-                           Rcap ms t (detaddrs ms t) \<and> Wcap ms t (detaddrs ms t)"
+                           Rcap ms t (detaddrs ms t) \<and> Wcap ms t (detaddrs ms t)
+                       \<and> \<not>n_dec ms t
+                       \<and> n ms t \<noteq> None 
+"
 (*(\<exists>j. s ms t = Some j)
                         \<and> (\<exists>i. n ms t = Some i)
                         \<and> (\<exists>k. v ms t = Some k)
@@ -715,7 +844,10 @@ definition "pre_S6 ms t \<equiv>
                         \<and> r ms t (CTRsync\<^sub>2 ms t) = 1
                         \<and>*)
 definition "pre_S7 ms t \<equiv>
-                          Rcap ms t (detaddrs ms t) \<and> Wcap ms t (detaddrs ms t)"
+                          Rcap ms t (detaddrs ms t) \<and> Wcap ms t (detaddrs ms t)
+                       \<and> \<not>n_dec ms t
+                       \<and> n ms t \<noteq> None 
+"
 (*(\<exists>j. s ms t = Some j)
                         \<and> (\<exists>i. n ms t = Some i)
                         \<and> (\<exists>k. v ms t = Some k)
@@ -786,11 +918,10 @@ lemmas pre_conds [simp] = pre_I1_def pre_I2_def pre_I3_def pre_I4_def pre_I5_def
 *)
 
 definition "init ms ps \<equiv>  (\<forall>t. (t<T_max)\<longrightarrow> pc ms t = I1
-                         \<and> n_alloc ms t = False
-                         \<and> s_alloc ms t = False
+                         \<and> n_dec ms t = False
+                         \<and> s_dec ms t = False
                          \<and> v ms t = None
                          \<and> n ms t = None
-                         \<and> s ms t = None
                          \<and> det ms t = []
                          \<and> CTRsync\<^sub>1 ms t = 0
                          \<and> CTRsync\<^sub>2 ms t = 0
@@ -822,138 +953,865 @@ definition "main_invariant_3 ms \<sigma> \<equiv> \<forall>k t t'. ( k<length (d
 *)
 
 (* Main Invariant *)
-definition "main_inv ms \<equiv>\<forall>t. (t\<le>T_max \<and> n_alloc ms t = True
-                                         \<and> n ms t \<noteq> None)\<longrightarrow>
-                                    own\<^sub>R ms (the (n ms t)) = {t}"
+definition "main_inv ms \<equiv>\<forall>t. (t\<le>T_max 
+                            \<and> n_dec ms t = True
+                            \<and> n ms t \<noteq> None)
+                  \<longrightarrow> own\<^sub>R ms (the (n ms t)) = {t}"
 
-lemmas new_main_inv [simp] = main_inv_def
+definition "main_inv_2 ms ps\<equiv> \<forall>loc. isfree_addr loc ps \<longrightarrow> own\<^sub>R ms loc = {}"
+definition "main_inv_3 ms ps\<equiv> \<forall>loc t. t\<notin>own\<^sub>R ms loc \<longrightarrow> own\<^sub>W ms loc \<noteq> Some t"
+
+
+
+lemma "main_inv_2 ms ps \<Longrightarrow> main_inv_3 ms ps \<Longrightarrow> isfree_addr loc ps \<Longrightarrow>
+          own\<^sub>R ms loc = {} \<Longrightarrow> own\<^sub>W ms loc = None"
+  apply (simp add:main_inv_2_def main_inv_3_def) 
+  by (metis empty_iff option.exhaust)
+
+
+
+definition "observation_lemma_ms ms ps \<equiv> \<forall>t loc .( (t\<le>T_max \<and> the(own\<^sub>W ms (loc)) = t)) \<longrightarrow>
+                              (loc \<in> (detaddrs ms t \<union> s_and_n ms t))"
+
+definition "observation_lemma_sig ms ps \<sigma> \<equiv> \<forall>t loc .( (t\<le>T_max \<and> the(own\<^sub>W ms (loc)) = t)
+                                                      \<or> \<not>isfree_addr loc ps) \<longrightarrow>
+                               (\<exists>val . cvd[C, val] \<sigma> \<longrightarrow> val \<noteq> loc)"
+
+                                              
+lemmas new_main_inv [simp] = main_inv_def main_inv_2_def main_inv_3_def
 
 (*supporting structure invariants*)
-definition "allocated_s_addr ms ps \<equiv> \<forall>t. (t\<le>T_max \<and> (s ms t)\<noteq>None)\<longrightarrow> \<not>(isfree_addr (the(s ms t)) ps)"
-definition "allocated_n_addr ms ps \<equiv> \<forall>t. (t\<le>T_max \<and> (n ms t)\<noteq>None)\<longrightarrow> \<not>(isfree_addr (the(n ms t)) ps)"
-definition "s_differs_from_n ms \<equiv> \<forall>t. (t\<le>T_max \<and> (s ms t)\<noteq>None \<and> (n ms t)\<noteq>None) \<longrightarrow> the(s ms t) \<noteq> the(n ms t)"
-definition "st_differs_from_sta ms\<equiv> \<forall>t t'. (t\<le>T_max \<and> t'\<le>T_max \<and> (s ms t)\<noteq>None \<and> (s ms t')\<noteq>None) 
-                                \<longrightarrow> the(s ms t) \<noteq> the(s ms t')"
-definition "nt_differs_from_nta ms \<equiv> \<forall>t t'. (t\<le>T_max \<and> t'\<le>T_max \<and> (n ms t)\<noteq>None \<and> (n ms t')\<noteq>None) 
-                                \<longrightarrow> the(n ms t) \<noteq> the(n ms t')"   
-definition "nt_differs_from_sta ms \<equiv> \<forall>t t'. (t\<le>T_max \<and> t'\<le>T_max \<and> (n ms t)\<noteq>None \<and> (s ms t')\<noteq>None) 
-                                \<longrightarrow> the(n ms t) \<noteq> the(s ms t')"
-definition "st_differs_from_nta ms \<equiv> \<forall>t t'. (t\<le>T_max \<and> t'\<le>T_max \<and> (s ms t)\<noteq>None \<and> (n ms t')\<noteq>None) 
-                                \<longrightarrow> the(s ms t) \<noteq> the(n ms t')"  
-definition "st_differs_from_detall ms\<equiv> \<forall>t ta. t\<le>T_max\<and>ta\<le>T_max\<and>s_alloc ms t \<longrightarrow> the(s ms t) \<notin> (detaddrs ms ta)"
-definition "nt_differs_from_detall ms\<equiv> \<forall>t ta. t\<le>T_max\<and>ta\<le>T_max\<and>n_alloc ms t \<longrightarrow> the(n ms t) \<notin> (detaddrs ms ta)"
+definition "allocated_s_addr ms ps \<equiv> \<forall>t. (t\<le>T_max \<and> (s ms t)\<noteq>None \<and> t\<in>own\<^sub>R ms (the(s ms t)))\<longrightarrow> \<not>(isfree_addr (the(s ms t)) ps)"
+definition "allocated_n_addr ms ps \<equiv> \<forall>t. (t\<le>T_max \<and> (n ms t)\<noteq>None \<and> (n_dec ms t))\<longrightarrow> \<not>(isfree_addr (the(n ms t)) ps)"
+definition "allocated_det_addr ms ps \<equiv> \<forall>t i. (t\<le>T_max \<and> det ms t\<noteq>[] \<and> i<length(det ms t))\<longrightarrow> \<not>(isfree_addr (det ms t ! i) ps)"
 
-definition "unique_allocs ms ps \<equiv> s_differs_from_n ms \<and> st_differs_from_sta ms \<and> nt_differs_from_nta ms
-                              \<and> nt_differs_from_sta ms \<and> st_differs_from_nta ms
-                              \<and> st_differs_from_detall ms \<and> nt_differs_from_detall ms"
+definition "allocated_rcuandC_addr ms ps \<equiv> (\<not>(isfree_addr (C) ps)) \<and> (\<forall>i. i<T_max \<longrightarrow> \<not>(isfree_addr (rcu_0+i) ps))"
+
+definition "allocated_addresses ms ps \<equiv> allocated_s_addr ms ps \<and> allocated_n_addr ms ps \<and> 
+                                        allocated_det_addr ms ps \<and> allocated_rcuandC_addr ms ps"
+lemmas allocation_lemmas = allocated_addresses_def
+                           allocated_s_addr_def allocated_n_addr_def
+                           allocated_det_addr_def allocated_rcuandC_addr_def
+
+definition "n_is_a_unique_loc ms \<equiv> \<forall>t ta. (t\<le>T_max \<and> ta\<le>T_max \<and> ta\<noteq>t
+                                        \<and> n_dec ms t \<and> n ms t \<noteq> None) 
+                      \<longrightarrow> the(n ms t) \<notin> ({the(s ms ta),the(n ms ta)}\<union>detaddrs ms ta)"
+
+definition "n_is_a_unique_local_loc ms \<equiv> \<forall>t. (t\<le>T_max \<and> n_dec ms t \<and> n ms t \<noteq> None) 
+                      \<longrightarrow> the(n ms t) \<notin> ({the(s ms t)}\<union>detaddrs ms t)"
+
+definition "n_uniqueness ms \<equiv> n_is_a_unique_loc ms \<and> n_is_a_unique_local_loc ms"
+
+definition "s_loc_rule ms \<equiv> \<forall>t ta. (t\<le>T_max \<and> ta\<le>T_max 
+                                        \<and> s ms t \<noteq> None \<and> t\<in> own\<^sub>R ms (the(s ms t)))
+                      \<longrightarrow> the(s ms t) \<notin> (detaddrs ms ta)"
+
+
+definition "general_structure ms \<equiv> n_uniqueness ms \<and> s_loc_rule ms"
+                                       
+lemmas general_structure_lemmas = general_structure_def
+                                  n_uniqueness_def s_loc_rule_def
+                                  n_is_a_unique_loc_def n_is_a_unique_local_loc_def
+
+lemma s_allocs_differs_from_n_allocs:
+  " general_structure ms\<Longrightarrow> 
+(t\<le>T_max \<and> ta\<le>T_max\<and> n_dec ms ta \<and> n ms ta \<noteq> None) \<Longrightarrow>
+                      the(s ms t) \<noteq> the(n ms ta) "
+  apply (simp_all add:general_structure_lemmas) 
+  by metis
+
+
+
+
 
 lemma differences:
   assumes "s ms 0 = Some 5"
   and "s ms 1 = Some 4" 
   and "T_max = 1"
-shows "the(s ms 0) \<noteq> the(s ms 1)"
-  using assms by(simp add:st_differs_from_sta_def)
+shows "s ms 0 \<noteq> s ms 1"
+  using assms
+  by auto
 
 
 lemmas allocated [simp] = allocated_n_addr_def
-                          s_differs_from_n_def 
-                          st_differs_from_sta_def
-                          nt_differs_from_nta_def
-                          nt_differs_from_sta_def
-                          st_differs_from_nta_def
-                          st_differs_from_detall_def
-                          nt_differs_from_detall_def
-                          unique_allocs_def
+
+lemma ms_observation_lemma_Correctness_supp_1:
+  assumes "preCond ms ps \<sigma> (pc ms t) t"
+  and "t \<le> T_max"
+  and "ta \<le> T_max"
+  and "step ms ps \<sigma> (pc ms t) t ms' ps' \<sigma>'"    
+  and "general_structure ms"
+  and "ta \<noteq> t"
+shows "n ms ta = n ms' ta"
+  using assms
+  apply(simp add:step_def)
+  apply(simp add:preCond_def)
+  apply(case_tac "pc ms t", simp_all)
+  apply(simp_all add:abbr)
+  apply clarify
+  apply(simp_all add:general_structure_lemmas) apply(simp add:get_C_val_def)
+  apply(simp add:FAAZ_def)
+  apply(simp add: visible_writes_def) 
+  apply(subgoal_tac "n ms t \<noteq> n ms ta") prefer 2 
+  apply metis
+  apply clarsimp
+  apply(clarsimp)
+  apply clarify
+  apply(case_tac "snd (CAS t (a, b) (the (s ms t)) (the (n ms t)) \<sigma> ts')", simp_all)
+  apply(case_tac "CAS_succ ms t", simp_all add:abbr)
+  apply(clarsimp)
+  apply(case_tac "nondet_val ms t", simp_all add:abbr)
+  apply(case_tac "det ms t \<noteq> []", simp_all add:abbr)
+  apply(case_tac "CTRsync\<^sub>1 ms t < T_max", simp_all add:abbr)
+  apply(clarsimp)
+  apply(case_tac "CTRsync\<^sub>2 ms t < T_max", simp_all add:abbr)
+  apply(case_tac "r ms t (CTRsync\<^sub>2 ms t) = 0", simp_all add:abbr)
+  apply(clarsimp)
+  by(case_tac "reg ms t = Suc 0", simp_all add:abbr)
 
 
-lemma main_invariant_Correctness:
+lemma ms_observation_lemma_Correctness_supp_2:
+  assumes "preCond ms ps \<sigma> (pc ms t) t"
+  and "t \<le> T_max"
+  and "ta \<le> T_max"
+  and "step ms ps \<sigma> (pc ms t) t ms' ps' \<sigma>'"    
+  and "general_structure ms"
+  and "ta \<noteq> t"
+shows "s ms ta = s ms' ta"
+  using assms 
+  apply(simp add:step_def)
+  apply(simp add:preCond_def)
+  apply(case_tac "pc ms t", simp_all)
+  apply(simp_all add:abbr)
+  apply clarify
+  apply(simp_all add:general_structure_lemmas)apply(simp add:get_C_val_def)
+  apply(simp add:FAAZ_def)
+  apply(simp add: visible_writes_def) 
+  apply(subgoal_tac "n ms t \<noteq> n ms ta") prefer 2 
+  apply metis
+  apply clarsimp
+  apply(clarsimp)
+  apply clarify
+  apply(case_tac "snd (CAS t (a, b) (the (s ms t)) (the (n ms t)) \<sigma> ts')", simp_all)
+  apply(case_tac "CAS_succ ms t", simp_all add:abbr)
+  apply(clarsimp)
+  apply(case_tac "nondet_val ms t", simp_all add:abbr)
+  apply(case_tac "det ms t \<noteq> []", simp_all add:abbr)
+  apply(case_tac "CTRsync\<^sub>1 ms t < T_max", simp_all add:abbr)
+  apply(clarsimp)
+  apply(case_tac "CTRsync\<^sub>2 ms t < T_max", simp_all add:abbr)
+  apply(case_tac "r ms t (CTRsync\<^sub>2 ms t) = 0", simp_all add:abbr)
+  apply(clarsimp)
+  by(case_tac "reg ms t = Suc 0", simp_all add:abbr)
+
+lemma ms_observation_lemma_Correctness_supp_3:
+  assumes "preCond ms ps \<sigma> (pc ms t) t"
+  and "t \<le> T_max"
+  and "ta \<le> T_max"
+  and "step ms ps \<sigma> (pc ms t) t ms' ps' \<sigma>'"    
+  and "general_structure ms"
+  and "ta \<noteq> t"
+shows "det ms ta = det ms' ta"
+  using assms
+  apply(simp add:step_def)
+  apply(simp add:preCond_def)
+  apply(case_tac "pc ms t", simp_all)
+  apply(simp_all add:abbr)
+  apply clarify
+  apply(simp_all add:general_structure_lemmas)apply(simp add:get_C_val_def)
+  apply(simp add:FAAZ_def)
+  apply(simp add: visible_writes_def) 
+  apply(subgoal_tac "n ms t \<noteq> n ms ta") prefer 2 
+  apply metis
+  apply clarsimp
+  apply(clarsimp)
+  apply clarify
+  apply(case_tac "snd (CAS t (a, b) (the (s ms t)) (the (n ms t)) \<sigma> ts')", simp_all)
+  apply(case_tac "CAS_succ ms t", simp_all add:abbr)
+  apply(clarsimp)
+  apply(case_tac "nondet_val ms t", simp_all add:abbr)
+  apply(case_tac "det ms t \<noteq> []", simp_all add:abbr)
+  apply(case_tac "CTRsync\<^sub>1 ms t < T_max", simp_all add:abbr)
+  apply(clarsimp)
+  apply(case_tac "CTRsync\<^sub>2 ms t < T_max", simp_all add:abbr)
+  apply(case_tac "r ms t (CTRsync\<^sub>2 ms t) = 0", simp_all add:abbr)
+  apply(clarsimp)
+  by(case_tac "reg ms t = Suc 0", simp_all add:abbr)
+
+lemma "\<exists>a b. A ps prov = Some (a, b) \<Longrightarrow>prov \<in> dom(A ps)"
+  by (simp add: domIff)
+
+
+
+
+
+lemma ms_observation_lemma_Correctness_supp_4:
+  assumes "preCond ms ps \<sigma> (pc ms t) t"
+  and "t \<le> T_max"
+  and "ta \<le> T_max"
+  and "step ms ps \<sigma> (pc ms t) t ms' ps' \<sigma>'"    
+  and "general_structure ms"
+  and "ta \<noteq> t" 
+  and "the (own\<^sub>W ms loc) = ta"
+  and "\<not>isfree_addr loc ps"
+  and "loc \<noteq> hd (det ms t)"
+shows "the (own\<^sub>W ms' loc) = ta"
+  using assms apply (simp_all)
+  apply(simp add:step_def)
+  apply(simp add:preCond_def)
+  apply(case_tac "pc ms t", simp_all)
+  apply(simp_all add:abbr)
+  apply clarify
+  apply(simp_all add:general_structure_lemmas)
+  apply(subgoal_tac "loc\<noteq>loca", simp_all add:Rcap_def Wcap_def)  apply clarsimp apply(simp add:get_C_val_def)     
+  apply(simp add:FAAZ_def)
+  apply(simp add: visible_writes_def)  apply clarsimp 
+  apply clarsimp 
+  apply(simp add: visible_writes_def)   apply clarsimp
+  apply(case_tac "(snd (CAS t (a, b) (the (s ms t)) (the (n ms t)) \<sigma> ts'))", simp_all)
+  apply metis
+  apply(case_tac "CAS_succ ms t", simp_all add:abbr) apply clarsimp
+  apply(case_tac "nondet_val ms t", simp_all add:abbr) apply clarsimp
+  apply(case_tac "det ms t", simp_all add:abbr)apply clarify
+  apply(case_tac "CTRsync\<^sub>1 ms t < T_max", simp_all add:abbr) apply clarify
+  apply(case_tac "x = 0", simp_all)
+  apply(case_tac "CTRsync\<^sub>2 ms t < T_max", simp_all add:abbr)
+  apply(case_tac "r ms t (CTRsync\<^sub>2 ms t) = 0", simp_all add:abbr) apply clarify
+  apply(case_tac "v = 0", simp_all)
+  by(case_tac "reg ms t = 1", simp_all add:abbr)
+
+
+
+
+lemma ms_observation_lemma_Correctness:
   assumes "preCond ms ps \<sigma> pcr t"
+  and "t \<le> T_max"
   and "main_inv ms"
+  and "main_inv_2 ms ps"
+  and "main_inv_3 ms ps"
   and "pcr = pc ms t"
-  and "step ms ps \<sigma> pcr t ms' ps' \<sigma>'"
-  and "allocated_n_addr ms ps "
-  and "unique_allocs ms ps"
+  and "step ms ps \<sigma> pcr t ms' ps' \<sigma>'"    
+  and "general_structure ms"
   and "pcr' = pc ms' t"
-  and "pcr \<notin> {I8, I9, I10, I11, cas_res}"
-shows "main_inv ms'"
-  using assms apply (simp add:preCond_def step_def)
-  apply(case_tac[!] "pc ms t", simp_all add:abbr) 
-  defer 
-  apply metis 
-  apply metis apply(subgoal_tac "\<not>n_alloc ms t") apply(simp add:names_2) 
-  apply(elim conjE impE exE) 
-  apply(subgoal_tac "\<not>n_alloc ms t") prefer 2
+  and "ta \<le> T_max \<and> the (own\<^sub>W ms loc) = ta"
+  and "observation_lemma_ms ms ps"
+  and "ta \<noteq> t"
+shows "loc \<in> (detaddrs ms' ta \<union> s_and_n ms' ta)"
+  using assms 
+  apply(subgoal_tac "(det ms' ta) = (det ms ta)") prefer 2 
+  using ms_observation_lemma_Correctness_supp_3 
   apply force
-  apply(subgoal_tac "\<forall>t. t \<le> T_max \<and> n_alloc ms t \<and> (\<exists>y. n ms t = Some y) \<longrightarrow>
-             own\<^sub>R ms (the (n ms t)) = {t}") prefer 2 
-  apply blast
-  apply(subgoal_tac "\<forall>t. t\<noteq>t'
+  apply(subgoal_tac "the (s ms' ta) = the (s ms ta)") prefer 2 
+  using ms_observation_lemma_Correctness_supp_2 
+  apply force
+  apply(subgoal_tac "the (n ms' ta) = the (n ms ta)") prefer 2 
+  using ms_observation_lemma_Correctness_supp_1
+  apply force
+  apply(simp add:observation_lemma_ms_def)
+  by meson
 
-              defer
 
-  
-  
-  
-  
+lemma ms_observation_lemma_Correctness_2:
+  assumes "preCond ms ps \<sigma> pcr t"
+  and "t \<le> T_max"
+  and "main_inv ms"
+  and "main_inv_2 ms ps"
+  and "main_inv_3 ms ps"
+  and "pcr = pc ms t"
+  and "step ms ps \<sigma> pcr t ms' ps' \<sigma>'"    
+  and "general_structure ms"
+  and "pcr' = pc ms' t"
+  and "ta \<le> T_max \<and> the (own\<^sub>W ms loc) = ta"
+  and "observation_lemma_ms ms ps"
+  and "ta \<noteq> t"
+  and "\<not>isfree_addr loc ps"
+  and "loc \<noteq> hd (det ms t)"
+shows "observation_lemma_ms ms' ps'"
+  using assms 
+  apply(subgoal_tac "(det ms' ta) = (det ms ta)") prefer 2 
+  using ms_observation_lemma_Correctness_supp_3 
+  apply force
+  apply(subgoal_tac "the (s ms' ta) = the (s ms ta)") prefer 2 
+  using ms_observation_lemma_Correctness_supp_2 
+  apply force
+  apply(subgoal_tac "the (n ms' ta) = the (n ms ta)") prefer 2 
+  using ms_observation_lemma_Correctness_supp_1
+  apply force
+  apply(case_tac "the (own\<^sub>W ms loc) = ta") prefer 2
+  apply linarith 
+  apply(subgoal_tac "the (own\<^sub>W ms' loc) = ta") prefer 2 
+  using ms_observation_lemma_Correctness_supp_4 
+  apply meson
+  apply(subgoal_tac "loc \<in> (detaddrs ms' ta \<union> s_and_n ms' ta)") prefer 2
+  using ms_observation_lemma_Correctness apply blast
+  apply(simp add:observation_lemma_ms_def)
+  apply(simp add:observation_lemma_ms_def)
   sorry
 
 
 
 
-lemma from_int_to_I1:
-  assumes "init ms ps"
+
+
+
+
+
+
+
+lemma sigma_observation_lemma_Correctness:
+  assumes "preCond ms ps \<sigma> (pc ms t) t"
   and "wfs \<sigma>"
-  and "step ms ps \<sigma> I1 1 ms' ps' \<sigma>'"
-shows "pc ms' 1 = I2"
-  using assms apply(simp add:step_def init_def)
-  by(simp add:v_allocation_def)
+  and "t \<le> T_max"
+  and "step ms ps \<sigma> (pc ms t) t ms' ps' \<sigma>'"    
+  and "general_structure ms"
+  and "observation_lemma_ms ms ps"
+  and "observation_lemma_sig ms ps \<sigma>"
+  and "main_inv ms"
+  and "main_inv_2 ms ps"
+  and "main_inv_3 ms ps"
+  and "cvd[C,vala] \<sigma>"
+shows "observation_lemma_sig ms' ps' \<sigma>'"
+  using assms apply (simp_all)
+  apply(simp add:preCond_def RCU.step_def)
+  apply(case_tac "pc ms t", simp_all add:abbr)
+  apply(simp add:covered_v_def general_structure_lemmas )
+  apply clarify
+  apply(unfold observation_lemma_sig_def observation_lemma_ms_def)
+  by (metis (full_types))+
 
-lemma check1:
-  assumes "preCond ms ps \<sigma> pcr t"
-  and "init ms ps"
-  and "t=1"
-  shows "Rcap ms t {}"
-  using preCond_def Rcap_def assms init_def
-  apply simp
-  apply(case_tac "pcr", simp_all add:init_def)
-  by (simp_all add: Rcap_def)
 
-lemma check2:
-  assumes "preCond ms ps \<sigma> pcr t"
-  and "init ms ps"
-  and "t=1"
-  shows "\<nexists>i.(t\<in>own\<^sub>R ms i) "
-  using assms check1 [where ms=ms and ps=ps and \<sigma>=\<sigma> and pcr=pcr and t=t] 
-  using Rcap_def by auto
 
-lemma check3:
+lemma ms_observation_lemma_Correctnesssss:
+  assumes "preCond ms ps \<sigma> (pc ms t) t"
+  and "wfs \<sigma>"
+  and "t \<le> T_max"
+  and "step ms ps \<sigma> (pc ms t) t ms' ps' \<sigma>'"    
+  and "general_structure ms"
+  and "observation_lemma_ms ms ps"
+  and "observation_lemma_sig ms ps \<sigma>"
+  and "main_inv ms"
+  and "main_inv_2 ms ps"
+  and "main_inv_3 ms ps"
+  and "cvd[C,vala] \<sigma>"
+shows "observation_lemma_ms ms' ps'"
+  using assms apply (simp_all)
+  apply(simp add:preCond_def RCU.step_def)
+  apply(case_tac "pc ms t", simp_all add:abbr)
+  apply(simp add:covered_v_def general_structure_lemmas )
+  apply clarify
+  apply(unfold observation_lemma_sig_def observation_lemma_ms_def)
+  apply(subgoal_tac "\<forall>loc t. t\<le>T_max \<and> own\<^sub>W ms' loc  = Some t
+  \<longrightarrow> loc\<in>(detaddrs ms' t \<union> s_and_n ms' t) ") 
+  sorry
+
+
+
+
+
+
+
+
+
+
+
+lemma main_invariant_Correctness:
   assumes "preCond ms ps \<sigma> pcr t"
-  and "pcr = I14"
-  and "det ms t=[]"
-shows "\<nexists>i.(t\<in>own\<^sub>R ms i) "
-  using assms preCond_def
-  apply simp apply (cases "pcr", simp_all)
-  by (simp add: Rcap_def)
+  and "t \<le> T_max"
+  and "main_inv ms"
+  and "main_inv_2 ms ps"
+  and "pcr = pc ms t"
+  and "step ms ps \<sigma> pcr t ms' ps' \<sigma>'"    
+  and "general_structure ms"
+  and "pcr' = pc ms' t"
+  and "observation_lemma_ms ms ps"
+  and "observation_lemma_sig ms ps \<sigma>"
+shows "main_inv ms'"
+  using assms apply (simp add:preCond_def step_def)
+  apply(case_tac[!] "pc ms t", simp_all add:abbr) 
+  apply(intro allI)
+  apply(intro impI) apply(elim conjE exE) apply(simp add:isfree_addr_def) 
+  apply (metis insert_not_empty option.sel) 
+  apply(intro allI)
+  apply(simp add:general_structure_lemmas)
+  apply metis
+  defer (*I8*)
+  defer (*I9*)
+  defer (*I11*)
+  apply(simp add:general_structure_lemmas)
+  apply metis 
+  apply(case_tac "CAS_succ ms t", simp_all)
+  apply(simp_all add:abbr)
+  defer (*R2*)
+  apply(simp add:general_structure_lemmas) apply(case_tac "nondet_val ms t = True", simp_all)
+  apply(simp_all add:abbr)
+  apply(case_tac "det ms t \<noteq> []", simp_all) 
+  apply(simp_all add:abbr)
+  apply(simp add:general_structure_lemmas)
+  apply (metis Diff_empty Diff_insert0 insert_absorb insert_iff)
+  apply(case_tac "CTRsync\<^sub>1 ms t < T_max", simp_all)
+  apply(simp_all add:abbr)
+  defer (*S3*)
+  apply(case_tac "CTRsync\<^sub>2 ms t < T_max", simp_all)
+  apply(simp_all add:abbr)
+  apply(case_tac "r ms t (CTRsync\<^sub>2 ms t) = 0", simp_all)
+  apply(simp_all add:abbr)
+  defer (*S6*)
+  apply(case_tac "reg ms t = Suc 0", simp_all)
+  apply(simp add:abbr)
+  apply(simp add:abbr)
+  apply(clarify) 
+  apply(simp add:get_C_val_def) 
+  apply(subgoal_tac "(snd (FAAZ t (a, b) \<sigma> ts')) \<noteq> the(n ms ta)", simp add:FAAZ_def) (*need this as pre_cond*)
   
-lemma check4:
-  assumes "preCond ms ps \<sigma> pcr t"
-  and "pcr = I14"
-  and "det ms t=[]"
-shows "\<nexists>i.(the(own\<^sub>W ms i) = t) "
-  using assms preCond_def
-  apply simp apply (cases "pcr", simp_all)
-  by (simp add: Wcap_def)
+        apply (metis option.sel)
+  defer
+  apply clarify
+  apply(subgoal_tac "own\<^sub>R ms (the(n ms ta)) = {ta}") prefer 2
+  apply(simp add:general_structure_lemmas) 
+  apply (metis option.sel)
+  apply(simp add:general_structure_lemmas)  
+  apply clarify
+  apply(case_tac "snd (CAS t (a, b) (the (s ms t)) (the (n ms t)) \<sigma> ts') ")
+  apply(subgoal_tac "n_dec ms' t = False") prefer 2
+  apply(simp add:general_structure_lemmas)
+  apply(simp add:general_structure_lemmas)  
+  apply (metis option.sel)
+  apply(simp add:general_structure_lemmas)  
+  apply (metis option.sel)                      
+  apply(simp add:general_structure_lemmas)  
+  apply clarify
+  apply(case_tac "b", simp_all) prefer 2 
+  apply (metis option.sel) 
+  apply (metis option.sel)                     
+  apply(simp add:general_structure_lemmas)
+  apply clarify apply(simp add:names_2)
+  apply (metis option.sel)                  
+  apply(simp add:general_structure_lemmas)
+  apply clarify
+  apply(case_tac "v", simp_all) prefer 2
+  apply (metis option.sel)
+  apply (metis option.sel)
+  apply(simp add: visible_writes_def) 
+  apply(simp add:observation_lemma_def general_structure_lemmas covered_v_def FAAZ_def)  
+  apply(simp add:Wcap_def)
+  by (metis option.sel)
+  
 
-lemma check5:
+
+
+
+lemma main_invariant_2_Correctness:
   assumes "preCond ms ps \<sigma> pcr t"
-  and "pcr = I14"
-  and "det ms t\<noteq>[]"
-  and "(the(own\<^sub>W ms i) = t)"
-shows "\<exists>a. (det ms t ! a) = i "
-  using assms preCond_def
-  apply simp apply (cases "pcr", simp_all add:Wcap_def)
-  apply clarify 
-  by blast
+  and "t \<le> T_max"
+  and "main_inv ms"
+  and "main_inv_2 ms ps"
+  and "pcr = pc ms t"
+  and "step ms ps \<sigma> pcr t ms' ps' \<sigma>'"       (*and "allocated_n_addr ms ps "     seems redundant*)
+  and "general_structure ms"
+  and "pcr' = pc ms' t"
+  and "observation_lemma \<sigma> ms"
+shows "main_inv_2 ms' ps'"
+  using assms apply simp
+  apply(simp add:step_def) apply(case_tac "pc ms t", simp_all add:abbr)     
+  apply(simp add:general_structure_lemmas preCond_def)
+  apply(elim conjE exE, intro allI impI)
+  apply(simp add:names_2)    
+  (*FAAZ*)
+  defer     
+  apply(simp add:general_structure_lemmas preCond_def)
+  apply(elim conjE exE, intro allI impI)
+  apply(simp add:names_2)       
+  apply(simp add:general_structure_lemmas preCond_def)
+  apply(elim conjE exE, intro allI impI)
+  apply(simp add:names_2)  
+  apply(case_tac "snd (CAS t (a, b) (the (s ms t)) y \<sigma> ts') ") prefer 2
+  apply simp
+  apply simp
+  apply(case_tac "CAS_succ ms t", simp_all)
+  apply(simp add:general_structure_lemmas preCond_def abbr)
+  apply(simp add:general_structure_lemmas preCond_def abbr)
+  apply(simp add:general_structure_lemmas preCond_def abbr)
+  apply(elim conjE exE, intro allI impI)
+  apply(simp add:names_2)       
+  apply(case_tac "nondet_val ms t", simp_all)
+  apply(simp add:general_structure_lemmas preCond_def abbr)
+  apply(simp add:general_structure_lemmas preCond_def abbr)
+  apply(case_tac "det ms t \<noteq> []", simp_all)
+  apply(simp add:general_structure_lemmas preCond_def abbr)
+  apply(simp add:general_structure_lemmas preCond_def abbr)
+  apply(simp add:general_structure_lemmas preCond_def abbr)
+  apply(elim conjE exE, intro allI impI)
+  apply(simp add:names_2)       
+  (*show that own\<^sub>R ms i \<in> det ms t \<longrightarrow> at some point is only held by {t}*)
+  defer
+  apply(simp add:general_structure_lemmas preCond_def abbr)
+  apply(case_tac "CTRsync\<^sub>1 ms t < T_max", simp_all)
+  apply(simp add:general_structure_lemmas preCond_def abbr)
+  apply(simp add:general_structure_lemmas preCond_def abbr)
+  apply(elim conjE exE, intro allI impI)
+  apply(simp add:names_2)     
+  apply(case_tac "CTRsync\<^sub>2 ms t < T_max", simp_all)
+  apply(simp add:general_structure_lemmas preCond_def abbr)
+  apply(simp add:general_structure_lemmas preCond_def abbr)
+  apply(case_tac "r ms t (CTRsync\<^sub>2 ms t) = 0", simp_all)
+  apply(simp add:general_structure_lemmas preCond_def abbr)
+  apply(simp add:general_structure_lemmas preCond_def abbr)
+  apply(simp add:general_structure_lemmas preCond_def abbr)
+  apply(elim conjE exE, intro allI impI)
+  apply(simp add:names_2)         
+  apply(case_tac "reg ms t = Suc 0", simp_all)
+  apply(simp add:general_structure_lemmas preCond_def abbr)
+  apply(simp add:general_structure_lemmas preCond_def abbr)
+  (*FAAZ*)
+  apply(simp add:general_structure_lemmas preCond_def abbr)
+  apply(elim conjE exE, intro allI impI)
+  apply(simp add:names_2)   
+   defer
+  
+  sledgehammer
+  oops
+
+
+
+lemma General_Structure_Correctness:
+  assumes "preCond ms ps \<sigma> pcr t"
+  and "t \<le> T_max"
+  and "main_inv ms"
+  and "main_inv_2 ms ps"
+  and "pcr = pc ms t"
+  and "step ms ps \<sigma> pcr t ms' ps' \<sigma>'"       
+  and "general_structure ms"
+  and "pcr' = pc ms' t"
+  and "observation_lemma \<sigma> ms"
+  and "\<exists>prov loc. prov \<notin> dom(A ps) \<and> isfree_addr loc ps"
+shows "general_structure ms'"
+  using assms apply simp
+  apply(simp add:step_def) apply(case_tac "pc ms t", simp_all add:abbr)     
+  apply(simp_all add:general_structure_lemmas preCond_def names_2)
+  apply metis
+  apply metis 
+  defer
+  apply metis 
+  defer
+  defer
+  defer
+  apply metis
+  defer
+  defer
+  apply(elim conjE exE)
+  apply(case_tac "b", simp_all)
+  apply(case_tac "nondet_val ms t", simp_all add:abbr)
+  apply(case_tac "det ms t = []", simp_all add:abbr)
+  defer
+  apply(case_tac "CTRsync\<^sub>1 ms t < T_max", simp_all add:abbr)
+  defer
+  apply(case_tac "CTRsync\<^sub>2 ms t < T_max", simp_all add:abbr)
+  apply(case_tac "r ms t (CTRsync\<^sub>2 ms t) = 0", simp_all add:abbr)
+  defer
+  apply(case_tac "reg ms t = Suc 0", simp_all add:abbr)
+  prefer 2
+  apply(simp add:FAAZ_def)
+  apply(simp add:allocated_addresses_def observation_lemma_def)
+  apply (metis option.sel)
+  apply(intro conjI impI) prefer 2
+  apply clarify
+  apply(case_tac "ta = t", simp_all) prefer 2
+  apply (metis option.sel) apply clarify
+  apply(intro conjI impI)
+  apply(subgoal_tac "y \<notin> alloc_addrs ps") prefer 2
+  apply blast
+  apply(subgoal_tac "the (s ms t) \<in> alloc_addrs ps") 
+  apply blast
+  apply(subgoal_tac "allocated_addresses ms ps", simp_all add:allocation_lemmas)
+  oops
+
+
+
+
+lemma Global_Correctness:
+  assumes "preCond ms ps \<sigma> pcr\<^sub>t t"
+  and "preCond ms ps \<sigma> pcr\<^sub>t\<^sub>' t'"  
+  and "pcr\<^sub>t = pc ms t"
+  and "pcr\<^sub>t\<^sub>' = pc ms t'"
+  and "t \<noteq> t'"
+  and "main_inv ms"
+  and "main_inv_2 ms ps"
+  and "step ms ps \<sigma> pcr\<^sub>t t ms' ps' \<sigma>'"       (*and "allocated_n_addr ms ps "     seems redundant*)
+  and "general_structure ms"
+  and "pcr' = pc ms' t"
+shows "preCond ms' ps' \<sigma>' pcr\<^sub>t\<^sub>' t'"
+  using assms apply simp
+  apply(simp add:step_def) apply(case_tac "pc ms t", simp_all add:abbr)     
+  apply(simp add:general_structure_lemmas preCond_def)
+  apply(case_tac "pc ms t'", simp_all add:abbr names_2) 
+  
+  apply metis   apply metis    apply metis    apply metis    apply metis    apply metis
+  apply metis   apply metis    apply metis    apply metis    apply metis    apply metis  
+  apply metis   apply metis    apply metis    apply metis    apply metis    apply metis  
+  apply metis   apply metis    apply metis    apply metis    apply metis        
+ 
+  apply(simp add:general_structure_lemmas preCond_def)
+  apply(case_tac "pc ms t'", simp_all add:abbr names_2)  
+ 
+  apply metis   apply metis    apply metis    apply metis    apply metis    apply metis
+  apply metis   apply metis    apply metis    apply metis    apply metis    apply metis  
+  apply metis   apply metis    apply metis    apply metis    apply metis    apply metis  
+  apply metis   apply metis    apply metis    apply metis    apply metis        
+  
+  apply(simp add:general_structure_lemmas preCond_def)
+  apply(case_tac "pc ms t'", simp_all add:abbr names_2)
+ 
+  apply metis   apply metis    apply metis    apply metis    apply metis    apply metis
+  apply metis   apply metis    apply metis    apply metis    apply metis    apply metis  
+  apply metis   apply metis    apply metis    apply metis    apply metis    apply metis  
+  apply metis   apply metis    apply metis    apply metis    apply metis  
+
+  (*existential complication*) defer
+  apply(simp add:general_structure_lemmas preCond_def) 
+  apply(case_tac "pc ms t'", simp_all add:abbr names_2)  
+ 
+  apply metis   apply metis    apply metis    apply metis    apply metis    apply metis
+  apply metis   apply metis    apply metis    apply metis    apply metis    apply metis  
+  apply metis   apply metis    apply metis    apply metis    apply metis    apply metis  
+  apply metis   apply metis    apply metis    apply metis    apply metis        
+  
+  apply(simp add:general_structure_lemmas preCond_def)
+  apply(case_tac "pc ms t'", simp_all add:abbr names_2)
+ 
+  apply metis   apply metis    apply metis    apply metis    apply metis    apply metis
+  apply metis   apply metis    apply metis    apply metis    apply metis    apply metis  
+  apply metis   apply metis    apply metis    apply metis    apply metis    apply metis  
+  apply metis   apply metis    apply metis    apply metis    apply metis  
+  
+  apply(simp add:general_structure_lemmas preCond_def)
+  apply(case_tac "pc ms t'", simp_all add:abbr names_2)
+ 
+  apply metis   apply metis    apply metis    apply metis    apply metis    apply metis
+  apply metis   apply metis    apply metis    apply metis    apply metis    apply metis  
+  apply metis   apply metis    apply metis    apply metis    apply metis    apply metis  
+  apply metis   apply metis    apply metis    apply metis    apply metis  
+  
+  (*existential complication, FAAZ*) defer
+  (*weak memory read s*)defer
+  
+  apply(simp add:general_structure_lemmas preCond_def)
+  apply(case_tac "pc ms t'", simp_all add:abbr names_2)
+ 
+  apply metis   apply metis    apply metis    apply metis    apply metis    apply metis
+  apply metis   apply metis    apply metis    apply metis    apply metis    apply metis  
+  apply metis   apply metis    apply metis    apply metis    apply metis    apply metis  
+  apply metis   apply metis    apply metis    apply metis    apply metis
+  
+  (*existential complication, CAS*)defer
+   
+  apply(simp add:general_structure_lemmas preCond_def)
+  apply(case_tac "pc ms t'", simp_all add:abbr names_2)  
+ 
+  apply metis   apply metis    apply metis    apply metis    apply metis    apply metis
+  apply metis   apply metis    apply metis    apply metis    apply metis    apply metis  
+  apply metis   apply metis    apply metis    apply metis    apply metis    apply metis  
+  apply metis   apply metis    apply metis    apply metis    apply metis
+   
+  apply(simp add:general_structure_lemmas preCond_def)
+  apply(case_tac "pc ms t'", simp_all add:abbr names_2)  
+ 
+  apply metis   apply metis    apply metis    apply metis    apply metis    apply metis
+  apply metis   apply metis    apply metis    apply metis    apply metis    apply metis  
+  apply metis   apply metis    apply metis    apply metis    apply metis    apply metis  
+  apply metis   apply metis    apply metis    apply metis    apply metis
+   
+  apply(simp add:general_structure_lemmas preCond_def)
+  apply(case_tac "pc ms t'", simp_all add:abbr names_2)  
+ 
+  apply metis   apply metis    apply metis    apply metis    apply metis    apply metis
+  apply metis   apply metis    apply metis    apply metis    apply metis    apply metis  
+  apply metis   apply metis    apply metis    apply metis    apply metis    apply metis  
+  apply metis   apply metis    apply metis    apply metis    apply metis
+
+  apply(case_tac "CAS_succ ms t", simp_all)
+  apply(simp add:general_structure_lemmas preCond_def)
+  apply(case_tac "pc ms t'", simp_all add:abbr names_2)  
+ 
+  apply metis   apply metis    apply metis    apply metis    apply metis    apply metis
+  apply metis   apply metis    apply metis    apply metis    apply metis    apply metis  
+  apply metis   apply metis    apply metis    apply metis    apply metis    apply metis  
+  apply metis   apply metis    apply metis    apply metis    apply metis
+  apply(simp add:general_structure_lemmas preCond_def)
+  apply(case_tac "pc ms t'", simp_all add:abbr names_2)
+  apply metis   apply metis    apply metis    apply metis    apply metis    apply metis
+  apply metis   apply metis    apply metis    apply metis    apply metis    apply metis  
+  apply metis   apply metis    apply metis    apply metis    apply metis    apply metis  
+  apply metis   apply metis    apply metis    apply metis    apply metis
+
+  apply(simp add:general_structure_lemmas preCond_def)
+  apply(case_tac "pc ms t'", simp_all add:abbr names_2)
+ 
+  apply metis   apply metis    apply metis    apply metis    apply metis    apply metis
+  apply metis   apply metis    apply metis    apply metis    apply metis    apply metis  
+  apply metis   apply metis    apply metis    apply metis    apply metis    apply metis  
+  apply metis   apply metis    apply metis    apply metis    apply metis 
+  
+  apply(simp add:general_structure_lemmas preCond_def)
+  apply(elim conjE impE exE)
+  apply(case_tac "b", simp_all)
+  apply(case_tac "pc ms t'", simp_all add:abbr names_2) 
+ 
+  apply metis   apply metis    apply metis    apply metis    apply metis    apply metis
+  apply metis   apply metis    apply metis    apply metis    apply metis    apply metis  
+  apply metis   apply metis    apply metis    apply metis    apply metis    apply metis  
+  apply metis   apply metis    apply metis    apply metis    apply metis 
+  apply(case_tac "pc ms t'", simp_all add:abbr names_2) 
+  apply metis   apply metis    apply metis    apply metis    apply metis    apply metis
+  apply metis   apply metis    apply metis    apply metis    apply metis    apply metis  
+  apply metis   apply metis    apply metis    apply metis    apply metis    apply metis  
+  apply metis   apply metis    apply metis    apply metis    apply metis
+
+  apply(case_tac "nondet_val ms t", simp_all)
+  apply(simp add:general_structure_lemmas preCond_def)
+  apply(case_tac "pc ms t'", simp_all add:abbr names_2)
+  
+  apply metis   apply metis    apply metis    apply metis    apply metis    apply metis
+  apply metis   apply metis    apply metis    apply metis    apply metis    apply metis  
+  apply metis   apply metis    apply metis    apply metis    apply metis    apply metis  
+  apply metis   apply metis    apply metis    apply metis    apply metis
+  apply(simp add:general_structure_lemmas preCond_def)
+  apply(case_tac "pc ms t'", simp_all add:abbr names_2)
+  apply metis   apply metis    apply metis    apply metis    apply metis    apply metis
+  apply metis   apply metis    apply metis    apply metis    apply metis    apply metis  
+  apply metis   apply metis    apply metis    apply metis    apply metis    apply metis  
+  apply metis   apply metis    apply metis    apply metis    apply metis
+  
+  apply(case_tac "det ms t \<noteq> []", simp_all)
+  apply(simp add:general_structure_lemmas preCond_def)
+  apply(case_tac "pc ms t'", simp_all add:abbr names_2)
+  
+  apply metis   apply metis    apply metis    apply metis    apply metis    apply metis
+  apply metis   apply metis    apply metis    apply metis    apply metis    apply metis  
+  apply metis   apply metis    apply metis    apply metis    apply metis    apply metis  
+  apply metis   apply metis    apply metis    apply metis    apply metis
+  apply(simp add:general_structure_lemmas preCond_def)
+  apply(case_tac "pc ms t'", simp_all add:abbr names_2)
+  apply metis   apply metis    apply metis    apply metis    apply metis    apply metis
+  apply metis   apply metis    apply metis    apply metis    apply metis    apply metis  
+  apply metis   apply metis    apply metis    apply metis    apply metis    apply metis  
+  apply metis   apply metis    apply metis    apply metis    apply metis
+  
+  (*existential complication, kill(x)*)defer
+  
+  apply(simp add:general_structure_lemmas preCond_def)
+  apply(case_tac "pc ms t'", simp_all add:abbr names_2)
+  
+  apply metis   apply metis    apply metis    apply metis    apply metis    apply metis
+  apply metis   apply metis    apply metis    apply metis    apply metis    apply metis  
+  apply metis   apply metis    apply metis    apply metis    apply metis    apply metis  
+  apply metis   apply metis    apply metis    apply metis    apply metis
+  
+  apply(case_tac "CTRsync\<^sub>1 ms t < T_max", simp_all)
+  apply(simp add:general_structure_lemmas preCond_def)
+  apply(case_tac "pc ms t'", simp_all add:abbr names_2)
+  
+  apply metis   apply metis    apply metis    apply metis    apply metis    apply metis
+  apply metis   apply metis    apply metis    apply metis    apply metis    apply metis  
+  apply metis   apply metis    apply metis    apply metis    apply metis    apply metis  
+  apply metis   apply metis    apply metis    apply metis    apply metis
+  apply(simp add:general_structure_lemmas preCond_def)
+  apply(case_tac "pc ms t'", simp_all add:abbr names_2)
+  apply metis   apply metis    apply metis    apply metis    apply metis    apply metis
+  apply metis   apply metis    apply metis    apply metis    apply metis    apply metis  
+  apply metis   apply metis    apply metis    apply metis    apply metis    apply metis  
+  apply metis   apply metis    apply metis    apply metis    apply metis
+  
+  (*existential complication, (rcu_0 + CTRsync\<^sub>1) weak memory read*)defer
+  
+  apply(case_tac "CTRsync\<^sub>2 ms t < T_max", simp_all)
+  apply(simp add:general_structure_lemmas preCond_def)
+  apply(case_tac "pc ms t'", simp_all add:abbr names_2)
+  
+  apply metis   apply metis    apply metis    apply metis    apply metis    apply metis
+  apply metis   apply metis    apply metis    apply metis    apply metis    apply metis  
+  apply metis   apply metis    apply metis    apply metis    apply metis    apply metis  
+  apply metis   apply metis    apply metis    apply metis    apply metis
+  apply(simp add:general_structure_lemmas preCond_def)
+  apply(case_tac "pc ms t'", simp_all add:abbr names_2)
+  apply metis   apply metis    apply metis    apply metis    apply metis    apply metis
+  apply metis   apply metis    apply metis    apply metis    apply metis    apply metis  
+  apply metis   apply metis    apply metis    apply metis    apply metis    apply metis  
+  apply metis   apply metis    apply metis    apply metis    apply metis
+  
+  apply(case_tac "r ms t (CTRsync\<^sub>2 ms t) = 0", simp_all)
+  apply(simp add:general_structure_lemmas preCond_def)
+  apply(case_tac "pc ms t'", simp_all add:abbr names_2)
+  
+  apply metis   apply metis    apply metis    apply metis    apply metis    apply metis
+  apply metis   apply metis    apply metis    apply metis    apply metis    apply metis  
+  apply metis   apply metis    apply metis    apply metis    apply metis    apply metis  
+  apply metis   apply metis    apply metis    apply metis    apply metis
+  apply(simp add:general_structure_lemmas preCond_def)
+  apply(case_tac "pc ms t'", simp_all add:abbr names_2)
+  apply metis   apply metis    apply metis    apply metis    apply metis    apply metis
+  apply metis   apply metis    apply metis    apply metis    apply metis    apply metis  
+  apply metis   apply metis    apply metis    apply metis    apply metis    apply metis  
+  apply metis   apply metis    apply metis    apply metis    apply metis
+  
+  defer
+
+  apply(case_tac "reg ms t = Suc 0", simp_all) 
+  apply(simp add:general_structure_lemmas preCond_def)
+  apply(case_tac "pc ms t'", simp_all add:abbr names_2)
+  
+  apply metis   apply metis    apply metis    apply metis    apply metis    apply metis
+  apply metis   apply metis    apply metis    apply metis    apply metis    apply metis  
+  apply metis   apply metis    apply metis    apply metis    apply metis    apply metis  
+  apply metis   apply metis    apply metis    apply metis    apply metis
+  apply(simp add:general_structure_lemmas preCond_def)
+  apply(case_tac "pc ms t'", simp_all add:abbr names_2)
+  apply metis   apply metis    apply metis    apply metis    apply metis    apply metis
+  apply metis   apply metis    apply metis    apply metis    apply metis    apply metis  
+  apply metis   apply metis    apply metis    apply metis    apply metis    apply metis  
+  apply metis   apply metis    apply metis    apply metis    apply metis
+
+(*weak memory guarantees needed, I think (maybe I'm wrong)*)
+  oops
+
+
+
+
+
+
+
+(*lemma test2:
+  assumes "wfs \<sigma>"
+  and "get_C_val ms \<sigma> t ms' \<sigma>'"
+  and "cvd[C,u] \<sigma>"
+shows "cvd[C,u] \<sigma>'"
+  using assms apply (simp add:get_C_val_def FAAZ_def) apply(clarify) 
+  apply(simp add:update_trans_def covered_v_def Let_def rev_app_def add_cv_def update_mods_def update_modView_def
+      update_thrView_def)
+  apply(unfold writes_on_def value_def lastWr_def) apply safe
+  apply (metis fst_conv var_def)
+  apply (metis fst_conv var_def visible_var)
+  apply (metis fst_conv var_def visible_var)
+  apply (metis fst_conv var_def)
+  apply(simp add:visible_writes_def tst_def var_def valid_fresh_ts_def)
+  apply(unfold writes_on_def value_def lastWr_def wfs_def var_def) apply safe
+  (*ts; is max, nempty \<and> finite*) defer
+  apply auto[1]    
+  apply(simp) apply(intro conjI)
+  apply (meson subset_iff visible_writes_in_writes)
+  apply presburger
+  apply (metis fst_conv)
+  apply (metis fst_conv var_def visible_var)
+  apply (metis fst_conv var_def visible_var)
+  apply (metis fst_conv)
+  (*ts; is max*) defer    
+  apply(simp) apply(intro conjI)
+  apply (meson subset_iff visible_writes_in_writes)
+  apply presburger
+  sorry*)
+
+
+
+
           
 (*
 OWNERSHIP IDEAS:
