Treiber Stack C11/MODEL.thy
@@ -1,0 +1,42 @@
+(*load stores value to a location in weak memory
+s=C \<longrightarrow> s.next = C.next
+v=*s \<longrightarrow> v = s.next.val
+n_star <--_t fst(A(n ms t))
+n_star =_t v+1
+n*=v+1 \<longrightarrow> n.next.val = v+1
+
+memory model:   ____________C____s____n________old__new_____________n2________________
+             ...|___||___||x52||x54||x56||___||x78||x80||___||___||x90||___||___||___|
+                |___||___||x78||x78||x80||___||_0_||_x_||___||___||___||___||___||___| ...
+                ____________C____s____n1_______old__new_____________n2________________
+             ...|___||___||_C_||_s_||_n1||___||x78||x80||___||___||x90||___||___||___|
+                |___||___||x80||___||x80||___||Nul||_1_||___||___||___||___||___||___| ...
+ 
+
+[(s ms t) :=  C] 
+[v <-_t (s ms t)]
+[fst(A(n ms t)) :=_t v+1]
+
+
+    ____                          ______
+    |__|  <-- Location            |0x52|
+C=  |__|  <-- C.next    (C.val)   |0x78|    <-- old.loc
+    ____                          ______
+    |__|  <-- Location            |0x54|
+s=  |__|  <-- s.next    (s.val)   |0x80|
+    ____                          ______
+    |__|  <-- Location = s.next   |0x80| 
+v=  |__|  <-- v.val               |__2_|
+    ____                          ______
+    |__|  <-- Location            |0x56|
+n=  |__|  <-- n.next    (n.val)   |0x80|
+
+
+
+rd_cap(i) \<noteq> {} \<longrightarrow> A(i) --\\<longrightarrow> none
+wr_cap(i) \<noteq> {} \<longrightarrow> A(i) --\\<longrightarrow> none
+wr_cap(i) \<noteq> {} \<longrightarrow> cannot acquire rd_cap(i)
+
+
+
+*)
